Context.dfy
@@ -1,0 +1,473 @@
+// objects are "contextually OK"
+
+include "Ownership-Lemmata.dfy"
+include "Klon.dfy"
+
+///////////////////////////////////////////////////////////////////////////////
+///////////////////////////////////////////////////////////////////////////////
+///////////////////////////////////////////////////////////////////////////////
+///////////////////////////////////////////////////////////////////////////////
+///COK / CallOK  (not yet in the right order)
+///Probablu should go off to another file?
+
+lemma COKAMFO(oo : Owner, context : set<Object>)
+  decreases oo
+  requires CallOK(oo, context)
+  requires CallOK(context)
+  ensures  CallOK(flatten(oo), context)
+{
+  reveal COK();
+  reveal CallOK();
+
+forall x <- oo ensures ( CallOK(flatten({x}), context) ) //by
+  {
+    assert COK(x, context);
+//    COKownerAMFOs(x, context);
+    assert CallOK(x.AMFO, context);
+    assert CallOK(flatten({x}), context);
+  }
+ assert CallOK(flatten(oo), context);
+}
+
+
+lemma COKowner(a : Object, context : set<Object>)
+  decreases a.AMFO
+  requires COK(a, context)
+  requires CallOK(context)
+  ensures  CallOK(a.owner, context)
+  // ensures  AllTheseOwnersAreFlatOK(a.AMFO - {a})
+  // ensures  AllTheseOwnersAreFlatOK(a.allExternalOwners())
+  // ensures  a.OwnersValid()
+{
+  reveal COK();
+  reveal CallOK();
+
+//COKAMFO(a.owner, context);
+
+  forall  oo <- a.owner ensures COK(oo,context) {
+    assert oo in context;
+    assert oo.Ready();
+    assert oo.Valid();
+    assert oo.AllOutgoingReferencesAreOwnership(context);
+    assert oo.Context(context);
+
+  }
+  assert forall  oo <- a.owner :: COK(oo,context);
+  assert CallOK(a.owner, context);
+
+}
+
+
+lemma COKownerAMFOs(a : Object, context : set<Object>)
+  decreases a.AMFO
+  requires COK(a, context)
+  requires CallOK(context)
+  ensures  CallOK(a.AMFO, context)
+  // ensures  AllTheseOwnersAreFlatOK(a.AMFO - {a})
+  // ensures  AllTheseOwnersAreFlatOK(a.allExternalOwners())
+  // ensures  a.OwnersValid()
+{
+  reveal COK();
+  reveal CallOK();
+
+  assert a.Context(context);
+  assert a.AMFO <= context;
+  assert (forall oo <- a.AMFO :: oo.Ready());
+
+forall  oo <- a.AMFO ensures COK(oo,context) {
+  assert oo in context;
+  assert oo.Ready();
+  assert oo.Valid();
+  assert oo.AllOutgoingReferencesAreOwnership(context);
+  assert oo.Context(context);
+
+}
+assert forall  oo <- a.AMFO :: COK(oo,context);
+assert CallOK(a.AMFO, context);
+
+}
+
+lemma CallOKAMFO(aa : Owner, context : set<Object>)
+  requires CallOK(aa, context)
+  requires CallOK(context)
+  ensures  forall a <- aa :: CallOK(a.AMFO, context)
+  ensures  forall a <- aa :: a.AMFO <= context
+{
+  reveal CallOK();
+  reveal COK();
+
+}
+
+
+lemma COKgetsDeclaredFields(a : Object, context : set<Object>)
+  requires COK(a, context)
+  ensures a.AllFieldsAreDeclared()
+{
+   reveal COK();
+   assert COK(a, context);
+   assert a.Valid();
+   assert a.AllFieldsAreDeclared();
+}
+
+
+lemma COKWiderContext2(a : Object, less : set<Object>, more : set<Object>)
+//given COK(a,less) get COK(a, more)
+  requires a in less
+  requires COK(a,less)
+  requires less <= more
+  ensures COK(a,more)
+{
+  //assert  (forall o <- (a.AMFO - {a}), ooo <- o.AMFO :: a.AMFO >= o.AMFO > ooo.AMFO);
+assert a.allExternalOwners() <= less by {
+   reveal COK();
+   assert COK(a,less);
+   assert a.Context(less);
+  //  assert a.allExternalOwners() <= less;
+   }
+assert a.allExternalBounds() <= less by {
+    reveal COK();
+    assert COK(a,less); }
+
+assert COK(a,less);
+reveal COK();
+
+assert TRIBBLE: (forall o <- a.AMFO, ooo <- o.AMFO :: a.AMFO >= o.AMFO >= ooo.AMFO)
+  by {
+    assert COK(a,less);    reveal COK();
+    assert a.Ready();
+    assert (forall o <- a.AMFO, ooo <- o.AMFO :: a.AMFO >= o.AMFO >= ooo.AMFO);
+  }
+
+SML(a.allExternalOwners(), less, more);
+SML(a.allExternalBounds(), less, more);
+
+
+var context := more;
+assert
+    && (a in context)
+    //&& (a.AMFO <= context)
+    //&& (a.AMFB <= context) //sgould be derivable, AMFB <= AMFO
+    && (a.AMFB <= a.AMFO <= context)
+    && (forall oo <- a.AMFO :: oo.Ready())
+    && (forall o <- a.AMFO, ooo <- o.AMFO :: a.AMFO >= o.AMFO >= ooo.AMFO)
+  //  && (a.TRUMP()||(a.Ready() && a.Valid()))
+    && (a.Ready())
+    && (a.Valid())
+    && (a.AllOutgoingReferencesAreOwnership(context))
+//    && (a.AllOutgoingReferencesWithinThisHeap(context))
+    && (a.Context(context))
+    && AllTheseOwnersAreFlatOK(a.AMFO - {a})
+    ;
+
+assert COK(a,more);
+
+}
+
+lemma COKExtraContext(a : Object, context : set<Object>, extra : set<Object>)
+  //requires a in context
+  requires COK(a,context)
+  ensures COK(a,context + extra)
+    { COKWiderContext(a, context, extra); }
+
+lemma COKWiderContext(a : Object, context : set<Object>, extra : set<Object>)
+  requires a in context
+  requires COK(a,context)
+  ensures COK(a,context + extra)
+{
+  reveal COK();
+  assert COK(a,context);
+  assert context <= (context + extra);
+  COKWiderContext2(a, context, context + extra);
+// //  assert  (forall o <- (a.AMFO - {a}), ooo <- o.AMFO :: a.AMFO >= o.AMFO > ooo.AMFO);
+//
+// var context := context + extra;
+// assert
+//     && (a in context)
+//     //&& (a.AMFO <= context)
+//     //&& (a.AMFB <= context) //sgould be derivable, AMFB <= AMFO
+//     && (a.AMFB <= a.AMFO <= context)
+//     && (forall oo <- a.AMFO :: oo.Ready())
+//     && (forall o <- (a.AMFO - {a}), ooo <- o.AMFO :: a.AMFO >= o.AMFO > ooo.AMFO)
+//   //  && (a.TRUMP()||(a.Ready() && a.Valid()))
+//     && (a.Ready())
+//     && (a.Valid())
+//     && (a.AllOutgoingReferencesAreOwnership(context))
+// //    && (a.AllOutgoingReferencesWithinThisHeap(context))
+//     && (a.Context(context))
+//
+//     && AllTheseOwnersAreFlatOK(a.AMFO - {a})
+//     ;
+}
+
+//rename to extra context
+lemma CallOKWiderContext(aa: set<Object>, context : set<Object>, extra : set<Object>)
+  requires aa <= context
+  requires CallOK(aa,context)
+  ensures CallOK(aa,context + extra)
+{
+  reveal CallOK();
+  forall a <- aa { COKWiderContext(a,context,extra); }
+}
+
+lemma CallOKWiderContext2(aa: set<Object>, less : set<Object>, more : set<Object>)
+  requires aa <= less <= more
+  requires CallOK(aa,less)
+  ensures CallOK(aa,more)
+{
+  reveal CallOK();
+  forall a <- aa { COKWiderContext2(a,less,more); }
+}
+
+
+
+lemma CallOKWiderFocus(aa: set<Object>, bb : set<Object>, context : set<Object>)
+  requires aa <= context
+  requires bb <= context
+  requires CallOK(aa,context)
+  requires CallOK(bb,context)
+  ensures  CallOK(aa+bb,context)
+{
+  reveal CallOK();
+  assert forall a <- (aa     ) :: COK(a,context);
+  assert forall a <- (     bb) :: COK(a,context);
+  assert forall a <- (aa + bb) :: COK(a,context);
+}
+
+
+lemma CallOKWiderFocus2(less: set<Object>, more : set<Object>, context : set<Object>)
+  requires less <= more <= context
+  requires CallOK(less,context)
+  requires CallOK((more - less), context)
+  ensures  CallOK(more,context)
+{
+  reveal CallOK();
+  assert forall a <- (less)        :: COK(a,context);
+  assert forall a <- (more - less) :: COK(a,context);
+  assert forall a <- (more)        :: COK(a,context);
+}
+
+
+
+///IF owners OK were also bounded by a (sub)heap, then
+///the reads clauses could just look over that whole subheap...
+///that way lies... seplogic?
+opaque predicate COK(a : Object, context : set<Object>) : (r : bool)
+//NOTE Pulled fields from COK - owners etc in context
+//  reads context`fields, context`fieldModes
+  reads a`fields, a`fieldModes
+
+  // reads (set x <- a.extra, xa <- x.AMFO :: xa)`fields
+  // reads (set x <- a.extra, xa <- x.AMFO :: xa)`fieldModes
+  // reads  a.extra`fields, a.extra`fieldModes
+
+  // reads (set o1 <- context, o2 <- o1.ValidReadSet() :: o2)`fields
+  // reads (set o1 <- context, o2 <- o1.ValidReadSet() :: o2)`fieldModes
+  ensures r ==> (a in context)
+ {
+//extraOK   && a.extra == {}  //extra not yet cloned
+
+    && (a in context)
+    //&& (a.AMFO <= context)
+    //&& (a.AMFB <= context) //sgould be derivable, AMFB <= AMFO
+    //
+    /// atuff below moved to Readdy()..
+    // && (a.AMFB <= a.AMFO <= context)
+    // && (forall oo <- a.AMFX :: oo.Ready())
+    // && (forall o <- (a.AMFX), ooo <- o.AMFO :: a.AMFO >= o.AMFO > ooo.AMFO)
+    //
+    //
+  //  && (a.TRUMP()||(a.Ready() && a.Valid()))
+    && (a.Ready())
+    && (a.Valid())
+    && (a.AllOutgoingReferencesAreOwnership(context))
+//    && (a.AllOutgoingReferencesWithinThisHeap(context))   ///should this be here??
+    && (a.Context(context))
+
+//    && AllTheseOwnersAreFlatOK(a.AMFX)   //point here is we don't want a loop  in the definitoin of the COK predicate I think()
+//KJX redo to be a.AllExternalOwners() (or AMXO?)
+//now surfaced by COKowner :-)
+//also check BoundsNeating, BoundsNeswtingFromReady, and AMFOsisAMFOs5
+//should it be within the context?? (or owners are within this heap doe sthat!)
+ }
+
+
+// method  {:verify false}  XXXCOKat(a : Object, n : string, context : set<Object>) returns ( r : Object )
+//   ensures r == a.fields[n]
+//   ensures COK(r,context)
+//   modifies {}
+// {
+//   r := COKat(a,n,context);
+// }
+
+function {:isolate_assertions} COKat(a : Object, n : string, context : set<Object>) : ( r : Object )
+     reads a`fields, a`fieldModes,  context`fields, context`fieldModes
+  requires COK(a,context)
+  requires CallOK(context)
+  requires n in a.fields
+  requires a.Ready()  //comes from COK?
+  requires a.AllOutgoingReferencesWithinThisHeap(context)
+  requires forall x <- context :: x.Ready() && x.AllOutgoingReferencesWithinThisHeap(context)
+
+  ensures r == a.fields[n]
+  ensures COK(r,context)
+  //modifies {}
+{
+  reveal COK(); reveal CallOK();
+  var r := a.fields[n];
+  assert COK(a,context);
+
+  assert (a.AllOutgoingReferencesAreOwnership(context));
+  assert (a.AllOutgoingReferencesWithinThisHeap(context));
+  assert (a.Context(context));
+
+  assert (r in context);
+  assert CallOK(context);
+  assert forall x <- context :: x.AllOutgoingReferencesAreOwnership(context);
+  assert forall x <- context :: x.AllOutgoingReferencesWithinThisHeap(context);
+  assert forall x <- context :: x.Context(context);
+  assert (r.AMFO <= context);
+  assert (forall oo <- r.AMFO :: oo.Ready());
+  assert (r.Ready() && r.Valid());
+  assert (r.AllOutgoingReferencesAreOwnership(context));
+  assert (r.AllOutgoingReferencesWithinThisHeap(context));
+  assert (r.Context(context));
+
+
+  assert  COK(r,context);
+
+  r
+}
+
+opaque predicate CallOK(aa : set<Object>, context : set<Object> := aa)
+  reads aa`fields, aa`fieldModes
+//  reads context`fields, context`fieldModes
+  // reads (set o1 <- context, o2 <- o1.ValidReadSet() :: o2)`fields
+  // reads (set o1 <- context, o2 <- o1.ValidReadSet() :: o2)`fieldModes
+{
+  forall a <- aa :: COK(a,context)
+}
+
+lemma COKfromHeapContextReady(o : Object, m : Klon)
+  requires o in m.oHeap
+  requires m.HeapContextReady()
+   ensures COK(o, m.oHeap)
+{
+ reveal COK();
+ }
+
+
+
+lemma {:isolate_assertions} CallOKfromHeapContextReady(m : Klon)
+  requires m.HeapContextReady()
+   ensures forall x <- m.oHeap :: x.Context(m.oHeap)
+   ensures CallOK(m.oHeap)
+{
+  reveal COK(), CallOK();
+  assert forall x <- m.oHeap :: (x.Ready() && x.Valid() && x.Context(m.oHeap)) by { assert  m.HeapContextReady(); }
+  assert forall a <- m.oHeap :: COK(a,m.oHeap);
+ }
+
+
+
+lemma CallOKtoSubset(aa :set<Object>, context : set<Object> := aa)
+  requires CallOK(aa, context)
+  ensures  aa <= context
+  {
+    reveal CallOK();
+    assert forall a <- aa :: COK(a,context);
+    reveal COK();
+    assert forall a <- aa :: a in context;
+    assert aa <= context;
+  }
+
+lemma CallOKNarrowFocus(nn : set<Object>, aa : set<Object>, context : set<Object> := aa)
+  requires CallOK(aa, context)
+  requires nn <= aa
+  ensures  CallOK(nn, context)
+  {
+    reveal CallOK();
+    assert forall a <- aa :: COK(a,context);
+    reveal COK();
+    assert forall a <- nn :: COK(a,context);
+  }
+
+
+lemma CallOKNarrowContext(aa : set<Object>, less : set<Object> := aa,  more : set<Object>)
+  requires less <= more
+  requires CallOK(aa, more)
+  requires forall a <- aa :: a.Context(less)
+   ensures CallOK(aa, less)
+  {
+    reveal CallOK();
+    reveal COK();
+    assert forall a <- aa :: COK(a,less);
+  }
+
+
+
+
+lemma COKNarrowContext(a : Object, less : set<Object>, more : set<Object>)
+  requires less <= more
+  requires COK(a, more)
+  requires a.AMFO <= less
+  requires a.Ready()
+  requires a.Context(less)
+  ensures  COK(a, less)
+{
+  reveal COK();
+}
+
+lemma COKfromCallOK(a : Object, focus : set<Object>, context : set<Object>  := focus)
+  requires CallOK(focus, context)
+  requires a in focus
+  ensures COK(a, context)
+  {
+    reveal CallOK();
+  }
+
+
+lemma CallOKfromCOK(a : Object, context : set<Object>)
+  requires COK(a, context)
+  ensures  CallOK({a}, context)
+  {
+    reveal CallOK();
+  }
+
+lemma RVfromCOK(a : Object, context : set<Object>)
+  requires COK(a, context)
+  ensures a.Ready()
+  ensures a.Valid()
+  ensures a.AMFO <= context
+  ensures (forall oo <- a.AMFO :: oo.Ready())
+  {
+    reveal COK();
+  }
+
+lemma RVfromCallOK(aa : set<Object>, context : set<Object>)
+  requires CallOK(aa, context)
+  ensures  (forall a <- aa :: a.Ready())
+  ensures  (forall a <- aa :: a.Valid())
+  ensures  (forall a <- aa :: a.AMFO <= context)
+  ensures  (forall a <- aa, oo <- a.AMFO :: oo.Ready())
+  {
+    reveal COK(), CallOK();
+  }
+
+
+lemma NothingShallComeOfNothing(aa : set<Object>, context : set<Object>)
+  requires aa == {}
+  ensures  CallOK(aa,context)
+  {
+    reveal CallOK();
+  }
+
+lemma OneMoreHeap(a : Object, m : Klon, m' : Klon)
+  requires COK(a, m'.oHeap)
+  requires m.from(m')
+  ensures a.Ready()
+  ensures a.Valid()
+  ensures (forall oo <- a.AMFO :: oo.Ready())
+  ensures COK(a, m.oHeap)
+  {
+    reveal COK();
+  }
