Example.dfy
@@ -1,0 +1,192 @@
+include "Object.dfy"
+
+method Main()
+{
+  var frame := new Object.make(fields({"counter"}), {}, {}, "frame");
+
+  frame.setn("counter", 0);
+  frame.setn("counter", 1 + frame.getn("counter"));
+
+}
+
+
+method NotMain()
+ {
+    var counter : nat := 0;
+    counter := counter + 1;
+ }
+
+const application : Owner := {};
+
+method LinkedList() {
+
+var list  := new Object.make(fields({"head", "tail"}), application, application, "list");
+
+var link0 := new Object.make(fields({"next", "data"}), {list}, {list}, "link0", {} );
+var link1 := new Object.make(fields({"next", "data"}), {list}, {list}, "link1", {} );
+var link2 := new Object.make(fields({"next", "data"}), {list}, {list}, "link2", {} );
+var link3 := new Object.make(fields({"next", "data"}), {list}, {list}, "link3", {} );
+
+ list.setf("head", link0); list.setf("tail", link3);
+
+ link0.setf("next", link1); link1.setf("next", link2); link2.setf("next", link3);
+
+}
+
+type RObject = r : Object? | (r != null) && r.Ready() witness *
+
+lemma Paper_NoIncomingPointers(f : RObject,
+  o : RObject,
+  t : RObject)
+
+  requires outside(f,o)
+  requires strictlyInside(t,o)
+
+  ensures f != null
+  ensures f is Object
+
+   ensures not(refOK(f,t))
+{}
+
+
+method Paper_add(a : nat, b : nat) {
+
+
+
+
+
+  var c := a + b;
+  print "c == ", c, "\n";
+
+
+}
+
+type Frame = Object
+type U = Owner
+
+predicate without(frame : Frame, u : U)  {
+  frame !in u
+}
+
+method drop(frame : Frame, u : U)
+ ensures without(frame, u)
+{
+  assume without(frame, u);
+}
+
+method {:isolate_assertions} {:timeLimit 30} Paper_Embedded_add(a : nat, b : nat, caller : Frame, u : U)
+    returns(frame : Frame) ensures without(frame, u)
+    requires caller.Ready()
+    requires u >= flatten({caller})
+  {
+      frame := new Object.make(fields({"a","b","c"}), {caller}, u, "", {});
+      frame.setn("a", a);
+      frame.setn("b", b);
+      frame.setn("c", frame.getn("a") + frame.getn("b"));
+      print "c == ",  frame.getn("c"), "\n";
+      drop(frame,u);
+  }
+
+
+
+
+method {:isolate_assertions} {:timeLimit 30} MakeList(caller : Frame, u : U)
+    returns(frame : Frame) ensures without(frame, u)
+    requires caller.Ready()
+    requires caller.bound == caller.owner
+    requires "ret" in caller.fieldModes.Keys
+    requires u >= flatten({  caller   })
+  {
+     frame := new Object.make(fields({"a"}), {caller}, u, "", {});
+
+     var list  := new Object.make(fields({"head"}), {caller}, u, "list", caller.bound);
+
+    assert forall o <- flatten({list}) :: o.Ready();
+    assert nuBoundsOK({list}, {});
+
+      var i     := new Object.make(fields({"next", "data"}), {list}, {list}, "i", {} );
+      var j     := new Object.make(fields({"next", "data"}), {list}, {list}, "j", {} );
+
+      frame.setf("list", list);
+      list.setf("head", i);
+      i.setf("next", j);
+
+      caller.setf("ret", frame.getf("list"));
+      drop(frame,u);
+  }
+
+
+
+method {:isolate_assertions} {:timeLimit 30} list_method(list : Object, caller : Frame, u : U)
+    returns(frame : Frame) ensures without(frame, u)
+//    requires ownerInside(caller.self, list.owner)
+    requires caller.Ready()
+    // requires caller.bound == caller.owner
+    // requires list.bound == list.owner
+    requires u >= flatten({  caller   })
+    requires AllReady({caller,list})
+    requires nuBoundsOK({caller},{caller})
+//    requires forall o : Object <- {caller,list} :: o.AMFB >= flatten({caller,list})
+    requires refOK(caller, list)
+  {
+     frame := new Object.make(fields({"self"}), {caller,list}, u, "", {caller,list});
+     assert refOK(frame, list);
+
+      var i     := new Object.make(fields({"next", "data"}), {list}, {list}, "i", {} );
+      var j     := new Object.make(fields({"next", "data"}), {list}, {list}, "j", {} );
+
+      frame.setf("list", list);
+      list.setf("head", i);
+      i.setf("next", j);
+
+      caller.setf("ret", frame.getf("list"));
+      drop(frame,u);
+  }
+
+
+
+
+
+predicate allCompatible(oo : Owner)
+{ forall a <- oo, b <- oo :: (a != b) ==> compatible(a,b) }
+
+
+predicate isThread(a : Object) reads a`fieldModes {"THRED" in a.fieldModes.Keys}
+
+
+predicate compatible(a : Object, b : Object)
+ reads a`fieldModes, b`fieldModes
+  { not(isThread(a) && isThread(b)) }
+
+type Thread = Object
+
+lemma {:isolate_assertions} {:timeLimit 30} ThreadSafe(ta : Thread, tb : Thread, a : Object, b : Object)
+   requires ta.Ready() && tb.Ready() && a.Ready() && b.Ready()
+   requires ta != tb
+   requires isThread(ta)
+   requires isThread(tb)
+   requires strictlyInside(a,ta)
+   requires strictlyInside(b,tb)
+  //  requires inside(a,ta)
+  //  requires inside(b,tb)
+   requires allCompatible(a.AMFO)
+   requires allCompatible(b.AMFO)
+    ensures not(refOK(a,b))
+  {
+    assert not(compatible(ta,tb));
+    // assert a.AMFO >= ta.AMFO;
+    // assert ta in ta.AMFO;
+    // assert b.AMFO >= tb.AMFO;
+    // assert tb in tb.AMFO;
+    // assert ta in a.AMFO;
+    // assert tb in b.AMFO;
+
+    // if (a == b) {
+    //     assert ta in a.AMFO;
+    //     assert tb in a.AMFO;
+    //     assert allCompatible(a.AMFO);
+    //     assert false;
+    // }
+
+
+  }
