Main.dfy
@@ -1,0 +1,2654 @@
+include "Klon-HighLine.dfy"
+
+
+include "Ownership-Recursive.dfy"
+include "Printing.dfy"
+
+//  include "Z2.dfy" // birmnamwood14, isownedby  - fast
+include "SSO.dfy"
+
+
+
+
+
+const protoTypes : map<string, Mode> := fields({"t","a","b","c","d","e","k","l","m"})
+  // map["fa":= Evil]["fb":=Evil]  //wrong but will likely do for now?
+
+
+datatype Split = Split(within : OWNR, without : OWNR, m : Klon)
+
+function split(oo : OWNR, m : Klon) : Split
+  requires forall o <- oo :: m.objectReadyInKlown(o)
+{
+  Split( (set o <- oo | inside(o, m.o)), (set o <- oo | outside(o, m.o)), m)
+}
+
+
+lemma {:verify false} objectReadyToOwnerReadyInKlon(o : Object, m : Klon)
+  requires m.ownersReadyInKlown(o) || m.objectReadyInKlown(o)
+   ensures forall oo <- o.AMFX :: oo.Ready()
+   ensures forall oo <- o.AMFX :: oo.AMFO <= m.m.Keys
+   ensures forall oo <- o.AMFX :: m.objectReadyInKlown(oo)
+  {
+    o.ExtraReady();
+  }
+
+function map2vmap(m : map<Object,Object>) : vmap<Object,Object>
+  requires AllMapEntriesAreUnique(m)
+  { m }
+
+
+
+function  sporamfo(o : Object) : Owner {(set oo : Object <- o.owner, ooo : Object <- oo.AMFO :: ooo) + {o}}
+  //takes an object via it's owners to its AMFO
+function sporamfx(o : Object) : Owner {set oo : Object <- o.owner,   ooo : Object <- oo.AMFO :: ooo}
+  //takes an object via it's owners to its AMFX
+function sporamfb(o : Object) : Owner {set oo : Object <- o.bound,   ooo : Object <- oo.AMFO :: ooo}
+  //takes an object via it's owners to its AMFB
+function splatten(os : Owner) : Owner {(set oo : Object <- os,       ooo : Object <- oo.AMFO :: ooo)}
+  //takes an Owner via it's owners to its AMFO
+
+
+function sporrel(k : Object, m : Klon) : string
+  requires k.Ready()
+ {
+   if (k == m.o) then ("pivot  ")
+     else if (outside(k, m.o))
+       then ("outside")
+       else ("inside ")
+ }
+
+
+datatype PrintOptions = PrintOptions (
+  graph : string,
+  lines : string,
+  nodes : string,
+  extra : string
+)
+{
+  predicate lineOpt(c : char)   { (lines == "") || (c in lines) }
+  predicate nodeOpt(n : string) { (nodes == "") || (n == "") || (n[0] in nodes) }
+}
+
+
+method getPrintOptions(args : seq<string>) returns (pops : PrintOptions)
+{
+  var ALLLINEOPTS := "OoBbFMR";
+  var aa := args;
+  if (|args| < 2)
+     { print "got no arguments!!\n";
+       print "going with dahlia 9 _" + ALLLINEOPTS + " _c _extra...\n";
+       aa := ["dahlia", "9"];
+       }
+
+   var graph : string := "";
+   var lines : string := "";
+   var nodes : string := "";
+   var extra : string := "";
+
+   if (|aa| > 1) { graph := aa[1]; }
+   if (|aa| > 2) { lines := aa[2]; }
+   if (|aa| > 3) { nodes := aa[3]; }
+   if (|aa| > 4) { extra := aa[4]; }
+
+   print "graph = ", graph, "\n";
+   print "lines = ", lines, "\n";
+   print "nodes = ", nodes, "\n";
+   print "extra = ", extra, "\n";
+
+   pops := PrintOptions(graph, lines, nodes, extra);
+
+   print "ALLLINEOPTS:\n";
+   for x := 0 to |ALLLINEOPTS| {
+       var opt : char := ALLLINEOPTS[x];
+       print opt, " ", pops.lineOpt(opt), "\n";
+   }
+
+}
+
+method {:verify false} Main(args : seq<string>)
+{
+  print "Snick! Snack! Snock!\n";
+
+  var pops := getPrintOptions(args);
+
+
+  var t,a,b,c,d,e,k,l,m,os,oq, loutName := zandal0();
+
+ if (pops.graph == "0")
+    {
+      t,a,b,c,d,e,k,l,m,os,oq, loutName := zandal10();
+    }
+
+ if (pops.graph == "9")
+    {
+      t,a,b,c,d,e,k,l,m,os,oq, loutName := zandal9();
+    }
+
+ if (pops.graph == "b")
+    {
+      t,a,b,c,d,e,k,l,m,os,oq, loutName := zandal9bounded();
+    }
+
+ if (pops.graph == "l")
+    {
+      t,a,b,c,d,e,k,l,m,os,oq, loutName := zandalList();
+    }
+
+
+
+
+
+//KLON fields
+  // m : vmap<Object,Object>,    //the  klon map
+  // o : Object,                 //object being copied
+  // clowner : Owner,            //owner of the clone
+  // clbound : Owner,            //bound of the clone
+  // oHeap : set<Object>,        //heap
+  // o_amfx : Owner,             //was o. so the AMFX of o
+  // //  c_amfb : OWNR,              //epected flattened bound of the clone..
+  // c_amfx : Owner
+
+
+  var v : map<Object,Object> := map[
+    // t := t,
+    // a := a,
+    // b := k,
+    // c := l,
+    // d := m,
+    // e := e
+  ];
+
+  assume AllMapEntriesAreUnique(v);
+  var v' : vmap<Object,Object> := map2vmap(v);
+
+
+  var hq := oq;
+  var hs := os;
+
+
+//  print "WARNING WARNING KLON KLON KLON\n";
+  var km := Klon(v', b, k.owner, k.bound, hs, b.AMFX, flatten(k.owner) );
+
+  assert km.o == b;
+  assert km.o.Ready();
+  assert b in hs;
+  assert km.o in hs;
+  assert km.o in km.m.Keys;
+
+  ////////////////////////////////////////////////////////////////////
+  assume km.objectInKlown(km.o);
+  ////////////////////////////////////////////////////////////////////
+//  assume HighCalidFragilistic(km);
+  ///////////////////////////////////////////////////////////////
+
+//    assert forall k <- km.m.Keys :: HighLineKV(k, km.m[k], km);
+    assert forall x <- hq :: km.objectInKlown(x);
+    assert HQIK: forall x <- hq :: km.objectInKlown(x);
+    assert HQNN: forall x <- hq :: x != null;
+
+// printobjectset(hs);
+//
+// printrefs(hq);
+
+      print "\n\n//STARTGRAPH\n";
+      print "////////////////////////////////////////////////////////////////////////////////\n";
+      print "////////////////////////////////////////////////////////////////////////////////\n";
+      print "////////////////////////////////////////////////////////////////////////////////\n";
+      print "//  ", loutName, "\n";
+
+
+  print "\n\ndigraph dafny {\n";
+  // print "   rankdir=\"TB\";\n";
+  print "   rankdir=\"BT\";\n";
+  print "   layers=\"mapping:fields:owner:bound:amfo:bg\";\n";
+//  print "   concentrate=true;\n";
+  print "   node [shape=box]\n\n";
+  print "//===\n", pops.extra,"\n//===\n";
+
+        graphobjectset(hs, km, pops);
+
+        if (pops.lineOpt('M')) { graphmapping(km.m, pops); }
+
+        if (pops.lineOpt('R')) {    graphrefs(hq, pops); }
+
+
+ print "}\n\n\n";
+
+    print "//ENDGRAPH\n";
+    print "////////////////////////////////////////////////////////////////////////////////\n";
+    print "///////////////////////////////////////////////////////////////////////////////\n";
+    print "////////////////////////////////////////////////////////////////////////////////\n";
+
+  print "\n\n//done\n";
+
+}
+
+ method {:verify false} do_object(o : Object, m : Klon)
+   requires m.objectReadyInKlown(o)
+   requires HighCalidFragilistic(m)
+ {
+   var spl := split(o.AMFO, m);  //WARNING WILL ROBINSON!!!
+   print o.nick;
+   print "  AMFO=", ffmtnickset(o.AMFO);
+   print "  within=", ffmtnickset(spl.within);
+   print "  without=", ffmtnickset(spl.without);
+
+   if (spl.within == {})
+     { print " (only outside, skipping)\n"; return; }
+    else { nl(); }
+
+    print "   processing..\n";
+    print "   within " + o.nick, "  AMFO=", ffmtnickset(o.AMFO), "\n";
+
+    var trimmed := o.AMFO - m.o.AMFO;
+    print "   trimmed ", ffmtnickset(trimmed), "\n";
+
+    var translated : SSO := {};
+
+    while trimmed != {}
+    {
+       var y: Object;
+       y :| y in trimmed;
+       trimmed := trimmed - {y};
+
+       print "      ", y.nick,"  AMFO=", ffmtnickset(y.AMFO);
+       if (y.AMFO >= m.o.AMFO)
+         {
+            var trans : Owner := mapThruKlon( (y.AMFO - m.o.AMFO), m ) +  ( m.m[m.o].AMFO );
+            translated := translated + {trans};
+            print "  tr=",ffmtnickset(trans),"\n";
+         } else {
+            translated := translated + {y.AMFO};  print "        (outside)\n";
+         }
+
+    }
+
+    var reconnected := translated + obj2sso( m.m[m.o] );
+    print "   done " + o.nick, " translated AMFO=", ffmtsso(reconnected),     "\n";
+    print "        " + o.nick, " direct     AMFO=", ffmtsso(obj2sso(m.m[o])), "\n";
+ }
+
+
+
+ method {:verify false}  do_object_mod(o : Object, m : Klon)
+   requires m.objectReadyInKlown(o)
+   requires HighCalidFragilistic(m)
+ {
+   var spl := split(o.AMFO, m);  //WARNING WILL ROBINSON!!!
+   print o.nick;
+   print "  AMFO=", ffmtnickset(o.AMFO);
+   print "  within=", ffmtnickset(spl.within);
+   print "  without=", ffmtnickset(spl.without);
+
+   if (spl.within == {})
+     { print " (only outside, skipping)\n"; return; }
+    else { nl(); }
+
+    print "   processing..\n";
+    print "   within " + o.nick, "  AMFO=", ffmtnickset(o.AMFO), "\n";
+
+    var trimmed := o.AMFO - m.o.AMFO;
+    print "   trimmed ", ffmtnickset(trimmed), "\n";
+
+    var translated : SSO := set y <- trimmed ::
+
+       if (y.AMFO >= m.o.AMFO) then
+         (
+            var trans : Owner := mapThruKlon( (y.AMFO - m.o.AMFO), m ) +  ( m.m[m.o].AMFO );
+            trans
+          ) else ( y.AMFO );
+
+    var reconnected := translated + obj2sso( m.m[m.o] );
+
+    print "   done " + o.nick, " translated AMFO=", ffmtsso(reconnected),     "\n";
+    print "        " + o.nick, " direct     AMFO=", ffmtsso(obj2sso(m.m[o])), "\n";
+ }
+
+
+
+ method {:verify false}  do_object_mod2(o : Object, m : Klon)
+   requires m.objectReadyInKlown(o)
+   requires HighCalidFragilistic(m)
+ {
+   var spl := split(o.AMFO, m);  //WARNING WILL ROBINSON!!!
+   print o.nick;
+   print "  AMFO=", ffmtnickset(o.AMFO);
+   print "  within=", ffmtnickset(spl.within);
+   print "  without=", ffmtnickset(spl.without);
+
+   if ((set x <- o.AMFO | inside(x, m.o)) == {})
+     { print " (only outside, skipping)\n"; return; }
+    else { nl(); }
+
+    print "   processing..\n";
+    print "   within " + o.nick, "  AMFO=", ffmtnickset(o.AMFO), "\n";
+
+    var trimmed := o.AMFO - m.o.AMFO;
+    print "   trimmed ", ffmtnickset(trimmed), "\n";
+
+    var translated : SSO := ( set y <- trimmed ::
+
+       if (y.AMFO >= m.o.AMFO) then
+         (mapThruKlon( (y.AMFO - m.o.AMFO), m ) +  ( m.m[m.o].AMFO )
+         ) else ( y.AMFO ) )
+    ;
+
+    var reconnected := translated + obj2sso( m.m[m.o] );
+
+    print "   done " + o.nick, " translated AMFO=", ffmtsso(reconnected),     "\n";
+    print "        " + o.nick, " direct     AMFO=", ffmtsso(obj2sso(m.m[o])), "\n";
+ }
+
+
+
+
+ method {:verify false} do_object_mod3(o : Object, m : Klon)
+   requires m.objectReadyInKlown(o)
+   requires HighCalidFragilistic(m)
+   requires m.SuperCalidFragilistic()
+    ensures m.Calid()   //no fucking idea wwhy this is failing,  but qutie curious!
+    ensures m.AllLinesCalid()
+ {
+   assert m.Calid();
+   assert m.AllLinesCalid();
+   var spl := split(o.AMFO, m);  //WARNING WILL ROBINSON!!!
+   print "o=",o.nick,"    m.o=", ffmtnickset(m.o.AMFO), "\n";
+
+   print "\n\n           AMFO=", ffmtnickset(o.AMFO);
+   print "\n           within=", ffmtnickset(spl.within);
+   print "\n          without=", ffmtnickset(spl.without);
+   print "\no.AMFO-m.o.AMFO**=", ffmtnickset(o.AMFO - m.o.AMFO);
+   print "\no.AMFO - {m.o}***=", ffmtnickset(o.AMFO - {m.o});
+   print "\no.AMFO -without  =", ffmtnickset(o.AMFO - spl.without);
+   print "\n   strictlyInside=", ffmtnickset(set x <- o.AMFO | strictlyInside(x, m.o));
+   print "\n           inside=", ffmtnickset(set x <- o.AMFO | strictlyInside(x, m.o));
+nl();
+
+   if ((set x <- o.AMFO | inside(x, m.o)) == {})
+      { print " (only outside, carrying on anyway to see what the FUCK happens)\n"; }
+//    { print " (only outside, skipping)\n"; return; }
+    else { nl(); }
+
+    print "   processing..\n";
+    print "   within " + fmtamfosso(o), "\n";
+    nl();
+
+
+
+
+    var reconnected := mapfo(o.AMFO, m);
+
+    if (reconnected != obj2sso(m.m[o]) )
+    {
+      print "FUCK fuck FUCK fuck FUCK fuck FUCK fuck FUCK fuck FUCK fuck FUCK fuck \n";
+      print "FUCK fuck FUCK fuck FUCK fuck FUCK fuck FUCK fuck FUCK fuck FUCK fuck \n";
+    }
+
+    print "   done " + o.nick, " translated  SSO=", ffmtsso(reconnected),             "\n";
+    print "        " + o.nick, " direct      SSO=", ffmtsso(obj2sso(m.m[o])),         "\n";
+    print "        " + o.nick, " mapfo_INNER SSO=", ffmtsso(mapfo_INNER(o.AMFO, m)),  "\n";
+    print "        " + o.nick, " mapfo_INNER+SSO=", ffmtsso(mapfo_INNER(o.AMFO, m) +  obj2sso(m.m[m.o])),  "\n";
+    print "        " + o.nick, " mapfo_orig  SSO=", ffmtsso(mapfo_orig(o.AMFO, m)),   "\n";
+
+    nl();
+
+    print "SPORRAN: ",  o.nick + " " + sporrel(o,m) + "                            rivet.AMFX=", ffmtnickset(o.AMFX); nl();
+    print "SPORRAN: ",  o.nick + " " + sporrel(o,m) + "                       sporamfx(rivet)=", ffmtnickset(sporamfx(o)); nl();
+    print "SPORRAN: ",  o.nick + " " + sporrel(o,m) + "                           trivet.AMFX=", ffmtnickset(m.m[o].AMFX); nl();
+    print "SPORRAN: ",  o.nick + " " + sporrel(o,m) + "                      sporamfx(trivet)=", ffmtnickset(sporamfx(m.m[o])); nl();
+    print "SPORRAN: ",  o.nick + " " + sporrel(o,m) + "             ownr2sso(sporamfx(trivet)=", ffmtsso(ownr2sso(sporamfx(m.m[o]))); nl();
+    print "SPORRAN: ",  o.nick + " " + sporrel(o,m) + "  ownr2sso(sporamfx(objThruKlon(o,m)))=", ffmtsso(ownr2sso(sporamfx(objThruKlon(o,m)))); nl();
+    print "SPORRAN: ",  o.nick + " " + sporrel(o,m) + "  ownr2sso(mapThruKlon(sporamfx(o),m))=", ffmtsso(ownr2sso(mapThruKlon(sporamfx(o),m))); nl();
+    print "SPORRAN: ",  o.nick + " " + sporrel(o,m) + "    ownr2sso(mapfoSide(sporamfx(o),m))=", ffmtsso(ownr2sso(mapfoSide(sporamfx(o),m))); nl();
+    print "SPORRAN: ",  o.nick + " " + sporrel(o,m) + "                  mapfo(sporamfx(o),m)=", ffmtsso(mapfo(sporamfx(o),m)); nl();
+
+ }
+
+
+lemma {:verify false}  GEownr(
+   p : SSO, w : SSO, mp : SSO , mw : SSO, m : Klon)
+   requires HighCalidFragilistic(m)
+       requires forall o <- concensso(p)  :: m.objectReadyInKlown(o)
+       requires forall o <- concensso(w)  :: m.objectReadyInKlown(o)
+       requires forall o <- concensso(mp) :: m.objectReadyInKlown(o)
+       requires forall o <- concensso(mw) :: m.objectReadyInKlown(o)
+       requires p >= w
+
+       requires mp == mapfo(concensso(p), m)
+       requires mw == mapfo(concensso(w), m)
+
+       ensures mp >= mw
+   {
+
+   }
+
+
+
+function parameterstk(os : Owner, m : Klon) : Owner
+  requires os <= m.m.Keys
+  reads m.oHeap, m.m.Values
+{ set o <- os :: m.m[o] }
+
+function mtk(os : Owner, m : Klon) : Owner
+  requires os <= m.m.Keys
+  reads m.oHeap, m.m.Values
+{ set o <- os :: m.m[o] }
+
+function mZk(os : Owner, m : Klon) : Owner
+  requires m.SuperCalidFragilistic()
+  requires os <= m.m.Keys
+  reads m.oHeap, m.m.Values
+  { if (os >= m.o.AMFO)
+     then (MINNER(os, m))
+     else (os) }
+
+function {:isolate_assertions}  msp(ko : OWNR, m : Klon) : OWNR
+  //map sporrelOWNR
+  requires ko <= m.m.Keys
+  requires m.SuperCalidFragilistic()
+  requires m.apoCalidse()
+  requires AllReady(ko)
+  requires isFlat(ko)
+     reads m.oHeap, m.m.Values
+ {
+   if (ko == m.o.AMFO) then (m.m[m.o].AMFO)
+     else if (not(ko >= m.o.AMFO))
+       then (ko)
+       else (MINNER(ko, m))
+ }
+
+
+
+function {:isolate_assertions}  pOb(k : Object, m : Klon) : OWNR
+  requires {k} <= m.m.Keys
+  requires m.SuperCalidFragilistic()
+  requires m.apoCalidse()
+  requires AllReady({k})
+     reads m.oHeap, m.m.Values
+ {
+  if (k == m.o) then (m.m[m.o].AMFO) else
+      (  if (outside(k,m.o))
+        then (sporamfo(k))
+        else (set z <- MINNER({k},m), zz9 <- sporamfo(z) :: zz9)  )
+ }
+
+
+
+function {:isolate_assertions}  pOW(ko : OWNR, m : Klon) : OWNR
+  ///this is too much of a hack
+   requires ko <= m.m.Keys
+  requires m.SuperCalidFragilistic()
+  requires m.apoCalidse()
+  requires AllReady(ko)
+  requires isFlat(ko)
+     reads m.oHeap, m.m.Values
+ {
+   if (ko == m.o.AMFO) then (m.m[m.o].AMFO)
+     else
+   if (ko == m.o.AMFB) then (m.m[m.o].AMFB)
+    else
+   if (ko == m.o.AMFX) then (m.m[m.o].AMFX)
+     else if (not(ko >= m.o.AMFO))
+       then (ko)
+       else (MINNER(ko, m))
+ }
+
+
+function MINNER(os : Owner, m : Klon) : Owner
+  requires m.SuperCalidFragilistic()
+  //compare mapfo_SIDEWAYS / _INNER
+  requires os <= m.m.Keys
+  reads m.oHeap, m.m.Values
+  {(set o <- (os - m.o.AMFO) :: m.m[o]) + m.m[m.o].AMFO }
+
+  /////////////////////////////////////////////////////////////////////////////////////////////////////////////
+
+
+function {:isolate_assertions}  zzX(k : Object, m : Klon) : OWNR
+  requires {k} <= m.m.Keys
+  requires m.SuperCalidFragilistic()
+  requires m.apoCalidse()
+  requires AllReady({k})
+     reads m.oHeap, m.m.Values
+ {
+  if (k == m.o) then (m.m[m.o].AMFO) else
+      (  if (outside(k,m.o))
+        then (sporamfo(k))
+        else (set z <- MINNER({k},m), zz9 <- sporamfo(z) :: zz9)  )
+ }
+
+
+
+
+
+
+  ///////////////////////////////////////////////////////////////////////////////////////////////////////////
+
+function pvtself(o : Object, m : Klon) : Owner {if (o == m.o) then (m.clowner+{m.m[o]}) else (mtk(o.self,m))}
+function pvtowner(o : Object, m : Klon) : Owner {if (o == m.o) then (m.clowner)          else (mtk(o.owner,m))}
+function pvtbound(o : Object, m : Klon) : Owner {if (o == m.o) then (m.clbound)          else (mtk(o.bound,m))}
+
+function xvtself(o : Object, m : Klon) : Owner {if (o == m.o) then ({})          else (mtk(o.self,m))}
+function xvtowner(o : Object, m : Klon) : Owner {if (o == m.o) then ({})          else (mtk(o.owner,m))}
+function xvtbound(o : Object, m : Klon) : Owner {if (o == m.o) then ({})          else (mtk(o.bound,m))}
+
+  ///////////////////////////////////////////////////////////////////////////////////////////////////////////
+
+ method   {:verify false}  do_object_mod4(k : Object, m : Klon)
+   requires m.objectReadyInKlown(k)
+   requires HighCalidFragilistic(m)
+   requires m.SuperCalidFragilistic()
+    ensures m.Calid()   //no fucking idea wwhy this is failing,  but qutie curious!
+    ensures m.AllLinesCalid()
+ {
+   var v := m.m[k];
+   print "^^^^^^^^^^^^^^^^^^^^^^^^^^^^^^^^^^^^^^^^^^^^^^^^^^^^^^^^^^^^^^^^^^^^^^^^^^^\n";
+   print "object ", sporrel(k,m), " ", k.nick, " ~> ", v.nick, "    ",ffmtnickset(k.AMFO),"~",ffmtnickset(v.AMFO),"      ", (v.AMFO  >= v.AMFB  >= k.AMFB);   nl();
+
+if (k == m.o) { print "PIBOTTTOTION  PIVOT\n"; } else { return; }
+
+print "clowner=", ffmtnickset(m.clowner), "  clbound=", ffmtnickset(m.clbound); nl();
+
+//    print "   k.owner=", ffmtnickset(k.owner);
+//    print " k.bound=", ffmtnickset(k.bound);nl();
+//    print " k.AMFO=", ffmtnickset(k.AMFO);
+//    print " k.AMFX=", ffmtnickset(k.AMFX);
+//    print " k.AMFB=", ffmtnickset(k.AMFB);
+//    print "  ", sporamfo(k)==k.AMFO," ", (sporamfx(k)==k.AMFX)," ", sporamfb(k)==k.AMFB;
+//    nl();
+//
+//
+//    print "   v.owner=", ffmtnickset(v.owner);
+//    print " v.bound=", ffmtnickset(v.bound);nl();
+//    print " v.AMFO=", ffmtnickset(v.AMFO);
+//    print " v.AMFX=", ffmtnickset(v.AMFX);
+//    print " v.AMFB=", ffmtnickset(v.AMFB);
+//    print "  ", sporamfo(v)==v.AMFO," ", (sporamfx(v)==v.AMFX)," ", sporamfb(v)==v.AMFB;
+//    nl();
+//
+
+  //  print " ", mtk(k.self, m) == v.self, " ", mtk(k.owner, m) == v.owner, " ", mtk(k.bound, m) == v.bound;
+  //  print " ", mZk(k.AMFO, m) == v.AMFO, " ", mZk(k.AMFX, m)  == v.AMFX, " ", mZk(k.AMFB, m) == v.AMFB;
+  //  nl();
+  //  nl();
+  //  print " ", msp(k.AMFO, m) == v.AMFO, " ", msp(k.AMFX, m)  == v.AMFX, " ", msp(k.AMFB, m) == v.AMFB;
+//   nl();
+
+   print "k  : ", ffmtnickset(k.self), " ", ffmtnickset(k.owner), " ", ffmtnickset(k.bound); nl();
+
+
+   print "v  : ", ffmtnickset(v.self), " ", ffmtnickset(v.owner), " ", ffmtnickset(v.bound); nl();
+   print "pvt: ", ffmtnickset(pvtself(k,m)), " ", ffmtnickset(pvtowner(k,m)), " ", ffmtnickset(pvtbound(k,m)); nl();
+
+   print "xvt: ", ffmtnickset(xvtself(k,m)), " ", ffmtnickset(xvtowner(k,m)), " ", ffmtnickset(xvtbound(k,m)); nl();
+
+
+
+   print "KLON ", ffmtnickset(m.clowner+{v}), " ", ffmtnickset(m.clowner), " ", ffmtnickset(m.clbound); nl();
+
+
+   print "pvt: ", pvtself(k,m) == v.self, " ", pvtowner(k,m) == v.owner, " ", pvtbound(k,m) == v.bound;
+   print "|", sporamfo(m.m[k]) == v.AMFO, " ", sporamfx(m.m[k])  == v.AMFX, " ", sporamfb(m.m[k]) == v.AMFB; nl();
+  //  print "mtk: ", mtk(k.self, m) == v.self, " ", mtk(k.owner, m) == v.owner, " ", mtk(k.bound, m) == v.bound;
+//    print "|", mtk(k.AMFO, m) == v.AMFO, " ", mtk(k.AMFX, m)  == v.AMFX, " ", mtk(k.AMFB, m) == v.AMFB; nl();
+//
+//
+//    print "mZk: ", mZk(k.self, m) == v.self, " ", mZk(k.owner, m) == v.owner, " ", mZk(k.bound, m) == v.bound;
+//    print "|", mZk(k.AMFO, m) == v.AMFO, " ", mZk(k.AMFX, m)  == v.AMFX, " ", mZk(k.AMFB, m) == v.AMFB; nl();
+//
+//    print "msp: ", msp(k.self, m) == v.self, " ", msp(k.owner, m) == v.owner, " ", msp(k.bound, m) == v.bound;
+//    print "|", msp(k.AMFO, m) == v.AMFO, " ", msp(k.AMFX, m)  == v.AMFX, " ", msp(k.AMFB, m) == v.AMFB; nl();
+// //
+//    print "pOb: ", pOb(k, m) == v.self, " ", pOb(k, m) == v.owner, " ", pOb(k, m) == v.bound;
+//    print "|", pOb(k, m) == v.AMFO, " ", pOb(k, m)  == v.AMFX, " ", pOb(k, m) == v.AMFB; nl();
+//
+//    print "pOW: ", pOW(k.self, m) == v.self, " ", pOW(k.owner, m) == v.owner, " ", pOW(k.bound, m) == v.bound;
+//    print "|", pOW(k.AMFO, m) == v.AMFO, " ", pOW(k.AMFX, m)  == v.AMFX, " ", pOW(k.AMFB, m) == v.AMFB; nl();
+
+   print "zzz: ", mtk(k.self, m) == v.self, " ", mtk(k.owner, m) == v.owner, " ", mtk(k.bound, m) == v.bound;
+   print "|", sporamfo(m.m[k]) == v.AMFO, " ", sporamfx(m.m[k])  == v.AMFX, " ", sporamfb(m.m[k]) == v.AMFB; nl();
+
+   print "zzz: ",ffmtnickset(mtk(k.self, m)), " ",ffmtnickset(mtk(k.owner, m)), " ",ffmtnickset(mtk(k.bound, m));
+   print "|",ffmtnickset(sporamfo(m.m[k])), " ",ffmtnickset(sporamfx(m.m[k])), " ",ffmtnickset(sporamfb(m.m[k])); nl();
+//
+//
+//    print "zz9: ", mtk(k.self, m) == v.self, " ", mtk(k.owner, m) == v.owner, " ", mtk(k.bound, m) == v.bound;
+//    print "|", splatten(mtk(k.owner,m)+{m.m[k]}) == v.AMFO, " ", splatten(mtk(k.owner,m)) == v.AMFX, " ", splatten(mtk(k.bound,m)) == v.AMFB; nl();
+//
+
+
+   print "zz8: ", mtk(k.self, m) == v.self, " ", mtk(k.owner, m) == v.owner, " ", mtk(k.bound, m) == v.bound;
+   print "|", splatten(m.m[k].owner)+{m.m[k]} == v.AMFO, " ", splatten(m.m[k].owner) == v.AMFX, " ", splatten(m.m[k].bound) == v.AMFB; nl();
+
+//    print "mfo:", mapfo(k.self, m) == ownr2sso(v.self), " ", mapfo(k.owner, m) == ownr2sso(v.owner), " ", mapfo(k.bound, m) == ownr2sso(v.bound);
+//    print "|", (mapfo(k.AMFO,m)) == ownr2sso(v.AMFO), " ", (mapfo(k.AMFX,m)) == ownr2sso(v.AMFX), " ", (mapfo(k.AMFB,m)) == ownr2sso(v.AMFB); nl();
+// //
+//4
+//    print "msp: ", mtk(k.self, m) == v.self, " ", mtk(k.owner, m) == v.owner, " ", mtk(k.bound, m) == v.bound;
+//    print "|", splatten(mtk(k.owner,m)+{m.m[k]}) == v.AMFO, " ", splatten(mtk(k.owner,m)) == v.AMFX, " ", splatten(mtk(k.bound,m)) == v.AMFB; nl();
+
+
+
+  //  ensures sporamfo(o) == splatten(o.owner)+{o}
+  //  ensures sporamfx(o) == splatten(o.owner)
+  //  ensures sporamfb(o) == splatten(o.bound)
+
+    var reconnected := mapfo(k.AMFO, m);
+
+    if (reconnected != obj2sso(m.m[k]) )
+    {
+      print "FUCK fuck FUCK fuck FUCK fuck FUCK fuck FUCK fuck FUCK fuck FUCK fuck \n";
+      print "FUCK fuck FUCK fuck FUCK fuck FUCK fuck FUCK fuck FUCK fuck FUCK fuck \n";
+    }
+
+
+
+
+   print "vvvvvvvvvvvvvvvvvvvvvvvvvvvvvvvvvvvvvvvvvvvvvvvvvvvvvvvvvvvvvvvvvvvvvvvvvvv\n\n";
+
+ }
+
+
+//{:timeLimit 60}
+lemma {:isolate_assertions} MapfoPLUS1(oo1 : OWNR, oo2 : OWNR, o : Object, m : Klon)
+   requires HighCalidFragilistic(m)
+   requires forall o <- oo1     :: m.objectReadyInKlown(o)
+   requires forall o <- oo2     :: m.objectReadyInKlown(o)
+    ensures mapfo(oo1 + oo2,m ) == mapfo(oo1,m) + mapfo(oo2,m)
+
+    requires oo2 == {o}
+   {
+     if (o in oo1) {
+      setfuck(oo1, oo2, o);
+      assert (oo1 + oo2) == (oo1 + {o}) == oo1;
+      assert mapfo(oo1 + oo2,m ) == mapfo(oo1,m) + mapfo(oo2,m);
+      return;
+     }
+     assert o !in oo1;
+   }
+
+
+lemma {:isolate_assertions} MapfoNULL(m : Klon)
+   requires HighCalidFragilistic(m)
+    ensures mapfo({}, m) == {}
+{}
+
+lemma {:isolate_assertions} SSOofNULL()
+    ensures ownr2sso({}) == {}
+{}
+
+lemma {:isolate_assertions} SSO_GT(oo1 : OWNR, oo2 : OWNR, m : Klon)
+   requires HighCalidFragilistic(m)
+   requires forall o <- oo1     :: m.objectReadyInKlown(o)
+   requires forall o <- oo2     :: m.objectReadyInKlown(o)
+   requires isFlat(oo1)
+   requires isFlat(oo2)
+   requires oo2 <= oo1
+    ensures ownr2sso(oo2) <= ownr2sso(oo1)
+   {}
+
+
+
+
+
+
+lemma {:isolate_assertions} MapfoPLUS2(oo1 : OWNR, oo2 : OWNR, o : Object, m : Klon)
+   requires HighCalidFragilistic(m)
+   requires forall o <- oo1     :: m.objectReadyInKlown(o)
+   requires forall o <- oo2     :: m.objectReadyInKlown(o)
+   requires isFlat(oo1)
+   requires isFlat(oo2)
+    requires oo2 == {o}
+    requires o in oo1
+     ensures oo2 <= oo1
+//     ensures mapfo(oo2,m) <= mapfo(oo1,m)
+   {
+
+assert oo2 <= oo1;
+assert ownr2sso(oo2) <= ownr2sso(oo1);
+// assert  (set o <- oo2 | inside(o, m.o)) <= (set o <- oo1 | inside(o, m.o));
+// assert ((set o <- oo1 | inside(o, m.o)) == {}) ==> ((set o <- oo2 | inside(o, m.o)) == {});
+
+assert (set o <- oo2 |  inside(o, m.o)) <= (set o <- oo1 |  inside(o, m.o));
+assert (set o <- oo2 | outside(o, m.o)) <= (set o <- oo1 | outside(o, m.o));
+
+
+if ((set o <- oo1 | inside(o, m.o)) == {})
+   {
+    assert mapfo(oo1,m) == ownr2sso(oo1);
+    assert oo2 <= oo1;
+    assert (set o <- oo2 | inside(o, m.o)) == {};
+    assert mapfo(oo2,m) == ownr2sso(oo2);
+    assert ownr2sso(oo2) <= ownr2sso(oo1);
+    assert mapfo(oo2,m) <= mapfo(oo1,m);
+    return;
+   }
+
+assert (set o <- oo1 | inside(o, m.o)) != {};
+
+// if ((set o <- oo2 | inside(o, m.o)) == {})
+//  {
+//
+//   assert mapfo(oo2,m) <= mapfo(oo1,m);
+//   return;
+//  }
+
+assert ((set o <- oo1 | inside(o, m.o)) != {}) && ((set o <- oo2 | inside(o, m.o)) != {});
+
+assert (set o <- oo2 |  inside(o, m.o)) <= (set o <- oo1 |  inside(o, m.o));
+assert (set o <- oo2 | outside(o, m.o)) <= (set o <- oo1 | outside(o, m.o));
+
+
+
+assert (oo2 - m.o.AMFO) <= (oo1 - m.o.AMFO);
+assert forall y <- (oo2 - m.o.AMFO) :: y in (oo1 - m.o.AMFO);
+
+assert mapfo_INNER(oo2,m) <= mapfo_INNER(oo1,m);
+
+assert (mapfo_INNER(oo2,m) + obj2sso(m.m[m.o])) <= (mapfo_INNER(oo1,m) + obj2sso(m.m[m.o]));
+
+assert mapfo(oo1,m) == (mapfo_INNER(oo1,m) + obj2sso(m.m[m.o]));
+assert mapfo(oo2,m) == (mapfo_INNER(oo2,m) + obj2sso(m.m[m.o]));
+
+//
+// assert
+//   (if ((set o <- oo2 | inside(o, m.o)) == {}) then ownr2sso(oo2) else (mapfo_INNER(oo2,m)) + obj2sso(m.m[m.o]))
+//   <=
+//   (if ((set o <- oo1 | inside(o, m.o)) == {}) then ownr2sso(oo1) else (mapfo_INNER(oo1,m)) + obj2sso(m.m[m.o]))
+//   ;
+
+
+
+assert mapfo(oo2,m) <= mapfo(oo1,m);
+
+   }
+
+lemma setfuck(oo1 : OWNR, oo2 : OWNR, o : Object)
+    requires oo2 == {o}
+    requires o in oo1
+     ensures oo1 + {o} == oo1
+     ensures oo1 + oo2 == oo1
+{}
+
+lemma setcrap(oo1 : OWNR, oo2 : OWNR, x : OWNR)
+    requires oo2 <= oo1
+     ensures (oo2+x) <= (oo1+x)
+{}
+
+
+lemma {:isolate_assertions} {:resource_limit 32000000} INSIDEOUT(oo : OWNR, m : Klon)
+   requires forall o <- oo :: m.objectReadyInKlown(o)
+   requires oo <= m.m.Keys
+   requires HighCalidFragilistic(m)
+    ensures ((set o <- oo | inside(o, m.o)) == {})  ==> (forall o <- oo :: outside(o, m.o))
+    ensures ((set o <- oo | inside(o, m.o)) == {}) <==  (forall o <- oo :: outside(o, m.o))
+
+    ensures ((set o <- oo | inside(o, m.o)) >  {})  ==> (exists o <- oo :: inside(o, m.o))
+    ensures ((set o <- oo | inside(o, m.o)) >  {}) <==  (exists o <- oo :: inside(o, m.o))
+
+    ensures ((set o <- oo | inside(o, m.o)) >  {})  ==> (not (forall o <- oo :: outside(o, m.o)))
+    ensures ((set o <- oo | inside(o, m.o)) >  {}) <==  (not (forall o <- oo :: outside(o, m.o)))
+ {}
+
+lemma {:isolate_assertions} MapfoEQ(oo1 : OWNR, oo2 : OWNR, m : Klon)
+   requires HighCalidFragilistic(m)
+   requires forall o <- oo1  :: m.objectReadyInKlown(o)
+   requires forall o <- oo2  :: m.objectReadyInKlown(o)
+    ensures (oo1 == oo2)  ==> (mapfo(oo1,m) == mapfo(oo2,m))
+ //   ensures (oo1 == oo2) <==  (mapfo(oo1,m) == mapfo(oo2,m))
+   {}
+
+
+lemma {:isolate_assertions} MapfoEQ2(o1 : Object, o2 : Object, m : Klon)
+   requires HighCalidFragilistic(m)
+   requires m.objectReadyInKlown(o1)
+   requires m.objectReadyInKlown(o2)
+    ensures (o1 == o2)  ==> (mapfo(o1.AMFO,m) == mapfo(o2.AMFO,m))
+  //  ensures (o1 == o2) <==  (mapfo(o1.AMFO,m) == mapfo(o2.AMFO,m))
+   {}
+
+
+ function {:isolate_assertions} {:timeLimit 20} mapfo_orig(oo : OWNR, m : Klon) : SSO
+   requires forall o <- oo :: m.objectReadyInKlown(o)
+   requires oo <= m.m.Keys
+   requires HighCalidFragilistic(m)
+    ensures                 m.o.AMFO <= m.m.Keys
+    ensures forall o <- oo :: o.AMFO <= m.m.Keys
+   reads oo, m.m.Keys, m.m.Values, m.oHeap
+ {
+   if ((set o : Object <- oo | inside(o, m.o)) == {}) then ownr2sso(oo) else
+
+    (( set y : Object <- (oo - m.o.AMFO) ::
+
+       if (y.AMFO >= m.o.AMFO) then
+         (mapThruKlon( (y.AMFO - m.o.AMFO), m ) +  ( m.m[m.o].AMFO )
+         ) else ( y.AMFO
+          )
+      ) + obj2sso(m.m[m.o]))
+
+ }
+
+
+
+
+
+lemma {:isolate_assertions} MAPFO_MAPFO_ORIG1(oo : OWNR, m : Klon)
+   requires forall o <- oo :: m.objectReadyInKlown(o)
+   requires oo <= m.m.Keys
+   requires HighCalidFragilistic(m)
+    ensures mapfo(oo,m) == mapfo_orig(oo,m)
+   { }
+
+
+lemma {:isolate_assertions}  {:timeLimit 120} MAPFO_MAPFO_ORIG2(oo : OWNR, m : Klon)
+   requires forall o <- oo :: m.objectReadyInKlown(o)
+   requires oo <= m.m.Keys
+   requires HighCalidFragilistic(m)
+    ensures mapfo_INNER(oo,m) == mapfo_INNER_NEW(oo,m)
+   { }
+
+lemma {:isolate_assertions}  MAPFO_MAPFO_INNER1(oo : OWNR, m : Klon)
+ //if there is at least one inside
+ //then we're calling INNER & added into m.m[m.o]
+   requires forall o <- oo :: m.objectReadyInKlown(o)
+   requires oo <= m.m.Keys
+   requires HighCalidFragilistic(m)
+   requires ((set o <- oo | inside(o, m.o)) > {})
+    ensures mapfo(oo,m) == (mapfo_INNER(oo,m) + obj2sso(m.m[m.o]))
+   { }
+
+//{:resource_limit 32000000}
+lemma {:isolate_assertions} MAPFO_MAPFO_INNER2(oo : OWNR, m : Klon)
+//if all items are outside m.o they go straight through
+   requires forall o <- oo :: m.objectReadyInKlown(o)
+   requires oo <= m.m.Keys
+   requires HighCalidFragilistic(m)
+
+   requires forall o <- oo :: outside(o, m.o)
+   requires oo !! m.o.AMFO
+    ensures mapfo(oo,m)       == ownr2sso(oo)
+//    ensures mapfo_INNER(oo,m) >= ownr2sso(oo)  //NOT this... *********
+  {}
+
+//
+// lemma {:isolate_assertions} MAPFO_MAPFO_INNER3(oo : OWNR, m : Klon)
+// //all items outside m.o go straight through!
+//    requires forall o <- oo :: m.objectReadyInKlown(o)
+//    requires oo <= m.m.Keys
+//    requires HighCalidFragilistic(m)
+//
+//     ensures forall o <- oo | strictlyInside(o, m.o) ::
+//        (mapfo_SIDEWAYS(o,m) in mapfo(oo,m))
+//   {
+//
+//   }
+
+
+
+lemma {:isolate_assertions}  MAPFO_MAPFO_INNER8(oo : OWNR, m : Klon, r : SSO, i : SSO)
+//incomplete.  does nothing.
+//OK now does the same as GT3i???
+   requires forall o <- oo :: m.objectReadyInKlown(o)
+   requires oo <= m.m.Keys
+   requires HighCalidFragilistic(m)
+   requires r == mapfo(oo,m)
+   requires i == mapfo_INNER(oo,m)
+
+   requires ((set o <- oo | inside(o, m.o)) > {})   //at least something is inside, so we go down that way. b
+
+   ensures mapfo(oo,m) == (mapfo_INNER(oo,m) + obj2sso(m.m[m.o]))
+   { }
+
+// lemma {:isolate_assertions} {:timeLimit 20} MAPFO_MAPFO_INNER9(oo : OWNR, m : Klon)
+//  //DOESNT, SHOULDNT, CANT WORK. THIS IS A BIT STUPID INNIT??
+//    requires forall o <- oo :: m.objectReadyInKlown(o)
+//    requires oo <= m.m.Keys
+//    requires HighCalidFragilistic(m)
+//
+//    requires ((set o <- oo | outside(o, m.o)) > {})
+//    // ensures mapfo(oo,m) == (mapfo_INNER(oo,m) + obj2sso(m.m[m.o]))
+//    {
+//     assert forall o <- oo :: outside(o, m.o);
+//     assert forall o <- oo :: not(o.AMFO >= m.o.AMFO);
+//     assert not( outside(m.o, m.o) );
+//     assert not(m.o.AMFO <= oo);
+//
+//    }
+
+
+
+
+//{:resource_limit 32000000}
+lemma {:isolate_assertions} MAPFO_MAPFO_GT1(oo1 : OWNR, oo2 : OWNR, m : Klon)
+  //mapfo_SIDEWAYS maintains <= (modulo preconditions)
+   requires forall o <- oo1 :: m.objectReadyInKlown(o)
+   requires forall o <- oo2 :: m.objectReadyInKlown(o)
+   requires oo1 <= m.m.Keys
+   requires oo2 <= m.m.Keys
+   requires isFlat(oo1)
+   requires isFlat(oo2)
+   requires HighCalidFragilistic(m)
+   requires oo2 <= oo1
+   requires forall o <- oo1 :: (o !in m.o.AMFO) && (inside(o, m.o))
+    ensures forall o <- oo2 :: (o !in m.o.AMFO) && (inside(o, m.o))
+    ensures (set o <- oo2 :: mapfo_SIDEWAYS(o,m)) <=
+                     (set o <- oo1 :: mapfo_SIDEWAYS(o,m))
+  { }
+
+
+//{:resource_limit 32000000}
+lemma {:isolate_assertions} MAPFO_MAPFO_GT2(oo1 : OWNR, oo2 : OWNR, m : Klon)
+ //mapfo Inner maintains <=
+   requires forall o <- oo1 :: m.objectReadyInKlown(o)
+   requires forall o <- oo2 :: m.objectReadyInKlown(o)
+   requires oo1 <= m.m.Keys
+   requires oo2 <= m.m.Keys
+   requires isFlat(oo1)
+   requires isFlat(oo2)
+   requires HighCalidFragilistic(m)
+   requires oo2 <= oo1
+
+    ensures mapfo_INNER(oo2,m) <= mapfo_INNER(oo1,m)
+    ensures (mapfo_INNER(oo2,m) + obj2sso(m.m[m.o])) <= (mapfo_INNER(oo1,m) + obj2sso(m.m[m.o]))
+{}
+
+
+lemma {:isolate_assertions} MAPFO_MAPFO_GT2thru(oo : OWNR, ext : Object, m : Klon)
+   requires forall o <- oo :: m.objectReadyInKlown(o)
+   requires oo <= m.m.Keys
+   requires isFlat(oo)
+   requires HighCalidFragilistic(m)
+   requires not(ext in m.o.AMFO) //?????
+   requires not(ext.AMFO >= m.o.AMFO)
+   requires ext in oo
+    ensures ext.AMFO in mapfo_INNER(oo,m)
+{}
+
+
+
+lemma {:isolate_assertions} MAPFO_MAPFO_GT2thru2(oo1 : OWNR, oo2 : OWNR, ext : Object, m : Klon)
+   requires forall o <- oo1 :: m.objectReadyInKlown(o)
+   requires forall o <- oo2 :: m.objectReadyInKlown(o)
+   requires oo1 <= m.m.Keys
+   requires oo2 <= m.m.Keys
+   requires isFlat(oo1)
+   requires isFlat(oo2)
+   requires HighCalidFragilistic(m)
+   requires oo2 <= oo1
+
+   requires not(ext in m.o.AMFO) //?????
+   requires not(ext.AMFO >= m.o.AMFO)
+   requires ext in oo2
+    ensures ext in oo1
+    ensures ext.AMFO in mapfo_INNER(oo2,m)
+    ensures ext.AMFO in mapfo_INNER(oo1,m)
+{}
+
+
+
+lemma {:isolate_assertions} MAPFO_MAPFO_GT2thrall(oo1 : OWNR, oo2 : OWNR, ext : Object, m : Klon)
+   requires forall o <- oo1 :: m.objectReadyInKlown(o)
+   requires forall o <- oo2 :: m.objectReadyInKlown(o)
+   requires oo1 <= m.m.Keys
+   requires oo2 <= m.m.Keys
+   requires isFlat(oo1)
+   requires isFlat(oo2)
+   requires HighCalidFragilistic(m)
+   requires oo2 <= oo1
+
+   requires not(ext in m.o.AMFO) //?????
+   requires not(ext.AMFO >= m.o.AMFO)
+   requires ext in oo2
+    ensures ext in oo1
+    ensures ext.AMFO in mapfo_INNER(oo2,m)
+    ensures ext.AMFO in mapfo_INNER(oo1,m)
+{}
+
+
+
+
+lemma {:isolate_assertions} MAPFO_MAPFO_GT3(oo1 : OWNR, oo2 : OWNR, m : Klon)
+  //supposed to be mapfo maintains <=? in all cases?
+   requires forall o <- oo1 :: m.objectReadyInKlown(o)
+   requires forall o <- oo2 :: m.objectReadyInKlown(o)
+   requires oo1 <= m.m.Keys
+   requires oo2 <= m.m.Keys
+   requires isFlat(oo1)
+   requires isFlat(oo2)
+   requires HighCalidFragilistic(m)
+   requires oo2 <= oo1
+
+  //  ensures mapfo(oo2,m) <= mapfo(oo1,m)
+{
+  //if oo1 is all outside pivot, so must be oo2 - and yourdon.
+  if ((set o <- oo1 | inside(o, m.o)) == {})  //forall o <- oo1 :: outside(o, m.o)
+     {
+      assert ((set o <- oo2 | inside(o, m.o)) == {}); // //forall o <- oo1 :: outside(o, m.o)
+
+      assert ownr2sso(oo2) <= ownr2sso(oo1);
+      assert mapfo(oo2,m) <= mapfo(oo1,m);
+      return;
+     }
+
+    //oo1 does have something inside.
+    assert ((set o <- oo1 | inside(o, m.o)) > {});
+
+
+  //if set2 *also* has something inside then we're both going thru inner
+  if ((set o <- oo2 | inside(o, m.o)) > {})
+     {
+      assert ((set o <- oo2 | inside(o, m.o)) > {});
+      assert OO2IN: ((set o <- oo2 | inside(o, m.o)) > {});
+      assert ((set o <- oo1 | inside(o, m.o)) > {});
+      assert oo2 <= oo1;
+      MAPFO_MAPFO_GT2(oo1,oo2,m);
+      assert
+        (mapfo_INNER(oo2,m) + obj2sso(m.m[m.o]))
+           <= (mapfo_INNER(oo1,m) + obj2sso(m.m[m.o]));
+
+      MAPFO_MAPFO_GT3i(oo1,m);
+      assert ((set o <- oo2 | inside(o, m.o)) > {}) by { reveal OO2IN; }
+      MAPFO_MAPFO_GT3i(oo2,m);
+      assert mapfo(oo1,m) == (mapfo_INNER(oo1,m) + obj2sso(m.m[m.o]));
+      assert mapfo(oo2,m) == (mapfo_INNER(oo2,m) + obj2sso(m.m[m.o]));
+      MAPFO_MAPFO_GT2(oo1,oo2,m);
+      assert mapfo(oo2,m) <= mapfo(oo1,m);
+      return;
+     }
+
+  //at this poiint oo1 definitely HAS something inside and goes down thru INNER
+  //but oo2 DOES NOT.
+  assert oo2 <= oo1;
+  assert ((set o <- oo1 | inside(o, m.o)) >  {});
+  assert ((set o <- oo2 | inside(o, m.o)) == {});
+//  assert ((set o <- oo2 | outside(o,m.o)) == oo2);
+// assert forall o <- oo2 :: outside(o, m.o);
+
+
+MAPFO_MAPFO_GT3x(oo1,oo2,m);
+assert mapfo(oo2,m) <= mapfo(oo1,m);
+}
+
+
+lemma {:isolate_assertions} MAPFO_MAPFO_GT3i(oo : OWNR, m : Klon)
+ // if there is at least one on oo inside, mapfo is Inner+thingey
+   requires forall o <- oo :: m.objectReadyInKlown(o)
+   requires oo <= m.m.Keys
+   requires isFlat(oo)
+   requires HighCalidFragilistic(m)
+   requires (set o <- oo | inside(o, m.o)) > {}   //exists o <- oo :: inside(o, m.o)
+    ensures mapfo(oo,m) == (mapfo_INNER(oo,m) + obj2sso(m.m[m.o]))
+{
+  //YAY DAFNY!!
+  // INSIDEOUT(oo,m);
+  // assert exists o <- oo :: inside(o, m.o);
+  // assert (set o <- oo | inside(o, m.o)) > {};
+  // assert mapfo(oo,m) == (mapfo_INNER(oo,m) + obj2sso(m.m[m.o]));
+
+}
+
+
+
+lemma XLEM<T(==)>(e : T, s : set<T>)
+   requires e in s
+    ensures {e} <= s
+    ensures {e} > {}
+    ensures (set o  <- s | e == o :: o) > {}
+  {}
+
+lemma YLEM<T(==)>(e : T, s : set<T>)
+   requires e in s
+    ensures {e} <= s
+    ensures {e} > {}
+    ensures (set o  <- s | {o} <= s) > {}
+  {}
+
+lemma ELEM<T(==)>(e :set<T>, s : set<set<T>>)
+   requires e in s
+    ensures {e} <= s
+    ensures {e} > {}
+    ensures (set o  <- s | {o} <= s) > {}
+ {}
+
+lemma FUKSSO(oo : OWNR, sso : SSO)
+   requires oo in sso
+    ensures {oo} <= sso
+    ensures {oo} > {}
+    ensures (set o <- sso | o <= oo) > {}
+ {}
+
+lemma {:isolate_assertions} {:timeLimit 15} MAPFO_MAPFO_GT3j(oo : OWNR, m : Klon)
+ //one inside pivot into mapfo, at least one inside blivet out of mapfo
+   requires forall o <- oo :: m.objectReadyInKlown(o)
+   requires oo <= m.m.Keys
+   requires isFlat(oo)
+   requires HighCalidFragilistic(m)
+    ensures forall k <- m.m.Keys :: m.m[k].Ready()
+   requires (set o <- oo | inside(o, m.o)) > {}                 //exists o <- oo :: inside(o, m.o)
+    ensures (m.m[m.o].AMFO) in mapfo(oo,m)
+    ensures (set o <- mapfo(oo,m) | o  >= m.m[m.o].AMFO) > {}   //exists o <- mapfo(oo,m) :: o >= m.m[m.o].AMFO
+{
+   assert (set o <- oo | inside(o, m.o)) > {};
+   MAPFO_MAPFO_GT3i(oo,m);
+   assert mapfo(oo,m) == (mapfo_INNER(oo,m) + obj2sso(m.m[m.o]));
+  //  assert inside(m.m[m.o], m.m[m.o]);
+  //  assert m.m[m.o].Ready();
+  //  assert forall o <- m.m[m.o].AMFO :: o.Ready();
+  //  assert forall oo <- obj2sso(m.m[m.o]), o <- oo :: o.Ready();
+   assert (m.m[m.o].AMFO) in obj2sso(m.m[m.o]);
+   assert (m.m[m.o].AMFO) in mapfo(oo,m);
+   assert {m.m[m.o].AMFO} > {};
+   assert (set o <- obj2sso(m.m[m.o]) | o  >= m.m[m.o].AMFO) > {}; //FUCK
+   assert (set o <- mapfo(oo,m)       | o  >= m.m[m.o].AMFO) > {};
+}
+
+
+lemma {:isolate_assertions} MAPFO_MAPFO_GT3o(oo : OWNR, m : Klon)
+ //everyting outside pivot into mapfo, nothing inside blivet outside mapfo
+   requires forall o <- oo :: m.objectReadyInKlown(o)
+   requires oo <= m.m.Keys
+   requires isFlat(oo)
+   requires HighCalidFragilistic(m)
+   requires forall o : Object <- oo :: outside(o,m.o)
+    ensures forall r : Owner <- mapfo(oo,m) :: not(r >= m.o.AMFO)
+    ensures forall r : Owner <- mapfo(oo,m) :: not(r >= m.m[m.o].AMFO)
+{}
+
+
+lemma {:isolate_assertions} {:timeLimit 30} MAPFO_MAPFO_GT3x(oo1 : OWNR, oo2 : OWNR, m : Klon)
+//IF oo2 <= oo1, AND oo1 has something inside, and oo2 does not, then mapfo oo2 <= mapfo oo1
+   requires forall o <- oo1 :: m.objectReadyInKlown(o)
+   requires forall o <- oo2 :: m.objectReadyInKlown(o)
+   requires oo1 <= m.m.Keys
+   requires oo2 <= m.m.Keys
+   requires isFlat(oo1)
+   requires isFlat(oo2)
+   requires HighCalidFragilistic(m)
+   requires oo2 <= oo1
+
+   requires (set o <- oo1 | inside(o, m.o)) >  {}    //exists o <- oo1 :: inside(o, m.o)
+   requires (set o <- oo2 | inside(o, m.o)) == {}    //requires forall o <- oo2 :: outside(o, m.o)
+   ensures mapfo(oo2,m) <= mapfo(oo1,m)
+
+{
+
+  assert oo2 <= oo1;
+  assert (set o <- oo1 | inside(o, m.o)) >  {};
+  assert (set o <- oo2 | inside(o, m.o)) == {};
+
+
+  var unicorn :| (unicorn in oo1) && (unicorn !in oo2) && (inside(unicorn, m.o));
+
+    assert unicorn.AMFO >= m.o.AMFO;
+    MAPFO_MAPFO_GT3o(oo2,m);
+    assert forall r : Owner <- mapfo(oo2,m) :: not(r >= m.o.AMFO);
+    assert forall r : Owner <- mapfo(oo2,m) :: not(r >= m.m[m.o].AMFO);
+
+    assert forall r : Owner <- mapfo(oo2,m) :: not(r >= m.m[m.o].AMFO);
+    assert unicorn.AMFO >= m.o.AMFO;
+
+assert isFlat(unicorn.AMFO);
+assert unicorn.AMFO > {};
+assert (set o <- unicorn.AMFO | o.AMFO >= m.o.AMFO) > {};
+
+MAPFO_MAPFO_GT3j(unicorn.AMFO,m);
+assert (set o <- mapfo(unicorn.AMFO,m) | o  >= m.m[m.o].AMFO) > {};
+
+assert oo2 <= oo1;
+assert (unicorn in oo1);
+assert (unicorn !in oo2);
+
+var        bicorn := mapfo({unicorn},m);
+assert     bicorn <= mapfo(oo1,m);         //WHAT THE FUCKY FUCK?
+assert not(bicorn <= mapfo(oo2,m));
+
+ assert not(mapfo(oo1,m) <= mapfo(oo2,m));
+
+ assert mapfo(oo2,m) <= mapfo(oo1,m);
+
+
+
+//  assert forall x : OWNR <- mapfo(oo2,m) :: not(x >= m.o.AMFO) && not(x >= m.m[m.o].AMFO);  //pivot & blivet
+
+}
+
+
+method {:isolate_assertions} {:timeLimit 30} wrangle7()
+//sets up a full clone with sideways owner
+//pivot is b, external owner is e, orig is b,c,d, d has owner c & sideowner e, clone is k l m
+  returns (t : Object, a : Object, b : Object, c : Object, d : Object, e : Object,
+           k : Object, l : Object, m : Object,
+           os : set<Object>, oq : seq<Object>)
+ ensures t.Ready()
+ ensures a.Ready()
+ ensures b.Ready()
+ ensures c.Ready()
+ ensures d.Ready()
+ ensures e.Ready()
+ ensures k.Ready()
+ ensures l.Ready()
+ ensures m.Ready()
+ ensures AllReady(os)
+//  ensures inside(d,c)
+//  ensures inside(d,e)
+ {
+    print "wrangle7\n";
+
+    t := new Object.make(protoTypes, {},  {},"t");
+    a := new Object.make(protoTypes, {t}, {t}, "a");
+    b := new Object.make(protoTypes, {a}, {t,a}, "bP");   //pivot
+    c := new Object.make(protoTypes, {b}, {t,a,b}, "c");  //inside clone
+    e := new Object.make(protoTypes, {t}, {t}, "eQ");       //external "sideways" owner
+    d := new Object.make(protoTypes, {c,e}, {t,a,b,c,e}, "dX"); //inside pivot and side owner
+
+    k := new Object.make(protoTypes, {t}, {t}, "k¢b"); //top of coone - of b
+    l := new Object.make(protoTypes, {k}, {t,k}, "l¢c"); //clone of c
+
+            var m_context := {t,k,l,e};
+            var m_oo := {l,e};
+            var m_mb := m_oo;
+
+            assert m_context >= flatten(m_oo);
+            expect m_context >= flatten(m_oo);
+            assert flatten(m_oo) >= flatten(m_mb);
+            expect flatten(m_oo) >= flatten(m_mb);
+            assert AllReady(m_oo);
+            expect AllReady(m_oo);
+            assert (flatten(m_mb) >= collectBounds(flatten(m_oo)));
+            expect (flatten(m_mb) >= collectBounds(flatten(m_oo)));
+            // assume m_context >= flatten(m_oo) >= flatten(m_mb);
+            // assume AllReady(m_oo);
+            // assume (flatten(m_mb) >= collectBounds(flatten(m_oo)));
+
+     m := new Object.make(protoTypes, m_oo, m_context, "m¢d"); //clone of d...
+
+//     b := new Object.make(protoTypes, {},  {},"b");
+//     c := new Object.make(protoTypes, {},  {},"c");
+//     d := new Object.make(protoTypes, {},  {},"d");
+
+    // k := new Object.make(protoTypes, {},  {},"k");
+    // l := new Object.make(protoTypes, {},  {},"l");
+    // m := new Object.make(protoTypes, {},  {},"m");
+
+
+
+    os := {t, a, b, c, d, e, k, l, m};
+    oq := [t, a, b, c, d, e, k, l, m];
+
+nl();
+  var x : nat;
+  for x := 0 to |oq| { print fmtamfob(oq[x]), "\n"; }
+nl();
+
+
+
+print "m_context= ", ffmtnickset(m_context), "\n";
+print "m_oo= ", ffmtnickset(m_oo), "\n";
+print "flatten(m_oo)= ", ffmtnickset(flatten(m_oo)), "\n";
+print "m_mb= ", ffmtnickset(m_mb), "\n";
+print "flatten(m_mb)= ", ffmtnickset(flatten(m_mb)), "\n";
+print "collectBounds(flatten(m_oo))= ", ffmtnickset(collectBounds(flatten(m_oo))), "\n";
+
+print "ctxt>=flatten(m_oo)= ", (m_context >= flatten(m_oo)), "\n";
+print "flatten(m_oo)>=flatten(m_mb)= ", (flatten(m_oo) >= flatten(m_mb)), "\n";
+print "AllReady(m_oo)= ", AllReady(m_oo), "\n";
+print "flatten(m_mb) >= collectBounds(flatten(m_oo))= ", flatten(m_mb) >= collectBounds(flatten(m_oo)), "\n";
+
+
+
+
+
+//
+//     assert forall x <- os :: x.Ready() by {
+//
+//         assert t.Ready();`
+//         assert a.Ready();
+//         assert b.Ready();
+//         assert c.Ready();
+//         assert d.Ready();
+//         assert e.Ready();
+//         assert k.Ready();
+//         assert l.Ready();
+//         assert m.Ready();
+//
+//         assert t in os;
+//         assert a in os;
+//         assert b in os;
+//         assert c in os;
+//         assert d in os;
+//         assert e in os;
+//         assert k in os;
+//         assert l in os;
+//         assert m in os;
+//
+//         assert os == {t, a, b, c, d, e, k, l, m};
+//
+//      }
+
+
+    AllTheseFuckingObjectsAreReadyYouIdiot(t, a, b, c, d, e, k, l, m, os);
+
+
+    assert forall x <- os :: x.Ready();
+
+
+
+    print "wrdone7\n";
+ }
+
+
+
+method {:isolate_assertions} jandal8()
+//sets up a full-done clone *reentrantly*
+//otherwise compatible with wrangle - except klone owned by d  from
+//pivot is b, external owner is e, orig is b,c,d, d has owner c & sideowner e, clone is k l m BUT now owned by **d**
+  returns (t : Object, a : Object, b : Object, c : Object, d : Object, e : Object,
+           k : Object, l : Object, m : Object,
+           os : set<Object>, oq : seq<Object>)
+ ensures t.Ready()
+ ensures a.Ready()
+ ensures b.Ready()
+ ensures c.Ready()
+ ensures d.Ready()
+ ensures e.Ready()
+ ensures k.Ready()
+ ensures l.Ready()
+ ensures m.Ready()
+ ensures AllReady(os)
+//  ensures inside(d,c)
+//  ensures inside(d,e)
+ {
+    print "jandal8\n";
+
+    t := new Object.make(protoTypes, {},  {},"t");
+    a := new Object.make(protoTypes, {t}, {t}, "a");
+    b := new Object.make(protoTypes, {a}, {t,a}, "bP");   //pivot
+    c := new Object.make(protoTypes, {b}, {t,a,b}, "c");  //inside clone
+    e := new Object.make(protoTypes, {t}, {t}, "eQ");       //external "sideways" owner
+    d := new Object.make(protoTypes, {c,e}, {t,a,b,c,e}, "dX"); //inside pivot and side owner
+
+
+
+assert t.AMFO == {t};
+assert a.AMFO == {t,a};
+assert b.AMFO == {t,a,b};
+assert c.AMFO == {t,a,b,c};
+assert e.AMFO == {t,e};
+assert d.AMFO == {t,a,b,c,d,e};
+
+//
+// assert collectAllOwners(t) == {t};
+// assert collectAllOwners(a) == {t,a};
+// assert collectAllOwners(b) == {t,a,b};
+// assert collectAllOwners(c) == {t,a,b,c};
+// assert collectAllOwners(e) == {t,e};
+//
+// assert d.owner == {c,e};
+// assert ({d} + {c,e}) == {c,d,e};
+// assert (set xo <- d.owner, co <- collectAllOwners(xo) :: co) == (collectAllOwners(c) + collectAllOwners(e));
+// var oCE := (collectAllOwners(c) + collectAllOwners(e));
+// assert oCE == (collectAllOwners(c) + collectAllOwners(e)) == ({t,a,b,c} + {t,e}) == {t,a,b,c,e};
+//
+// assert ({d} + d.owner + oCE) ==  {t,a,b,c,d,e};
+// assert collectAllOwners(d) == ({d} + d.owner +  collectAllOwners(c) + collectAllOwners(e)); // == {t,a,b,c,d,e};
+// assert collectAllOwners(d) == {t,a,b,c,d,e};
+//
+//
+
+
+
+
+printAllOwnershipsAndBounds({d}, {t,a,b,c,d,e}, "k¢b");
+
+assert flatten({d}) == {t,a,b,c,d,e};
+            assert {t,a,b,c,d,e} >= flatten({d});
+            assert flatten({d}) >= flatten({d});
+            assert AllReady({d});
+            assert (flatten({d}) >= collectBounds(flatten({d})));
+    k := new Object.make(protoTypes, {d}, {t,a,b,c,d,e}, "k¢b"); //top of coone - of b
+
+/// assert k.AMFO == {t,a,b,c,d,e,k};
+
+printAllOwnershipsAndBounds({k}, {t,a,b,c,d,e,k}, "l¢c");
+
+assume flatten({k}) == {t,a,b,c,d,e,k};
+            assert {t,a,b,c,d,e,k} >= flatten({k});
+            assert flatten({k}) >= flatten({k});
+            assert AllReady({k});
+            assert (flatten({k}) >= collectBounds(flatten({k})));
+    l := new Object.make(protoTypes, {k}, {t,a,b,c,d,e,k}, "l¢c"); //clone of c
+
+/// assert l.AMFO == {t,a,b,c,d,e,k,l};
+
+            var m_context := {t,a,b,c,d,e,k,l};
+            var m_oo := {l,e};
+            var m_mb := m_oo;
+
+            // assert m_context >= flatten(m_oo);
+            // assert flatten(m_oo) >= flatten(m_mb);
+            // assert AllReady(m_oo);
+            // assert (flatten(m_mb) >= collectBounds(flatten(m_oo)));
+
+            assume flatten(m_oo) == {t,a,b,c,d,e,k,l};
+
+            assert m_context >= flatten(m_oo);
+            expect m_context >= flatten(m_oo);
+            assert flatten(m_oo) >= flatten(m_mb);
+            expect flatten(m_oo) >= flatten(m_mb);
+            assert AllReady(m_oo);
+            expect AllReady(m_oo);
+            assert (flatten(m_mb) >= collectBounds(flatten(m_oo)));
+            expect (flatten(m_mb) >= collectBounds(flatten(m_oo)));
+            // assume m_context >= flatten(m_oo) >= flatten(m_mb);
+            // assume AllReady(m_oo);
+            // assume (flatten(m_mb) >= collectBounds(flatten(m_oo)));
+
+printAllOwnershipsAndBounds(m_oo, m_context, "m¢d");
+
+     m := new Object.make(protoTypes, m_oo, m_context, "m¢d"); //clone of d...
+
+//assert m.AMFO == {t,a,b,c,d,e,k,l,m};
+
+
+//     b := new Object.make(protoTypes, {},  {},"b");
+//     c := new Object.make(protoTypes, {},  {},"c");
+//     d := new Object.make(protoTypes, {},  {},"d");
+
+    // k := new Object.make(protoTypes, {},  {},"k");
+    // l := new Object.make(protoTypes, {},  {},"l");
+    // m := new Object.make(protoTypes, {},  {},"m");
+
+
+
+    os := {t, a, b, c, d, e, k, l, m};
+    oq := [t, a, b, c, d, e, k, l, m];
+
+nl();
+  var x : nat;
+  for x := 0 to |oq| { print fmtamfob(oq[x]), "\n"; }
+nl();
+
+
+
+
+//
+//     assert forall x <- os :: x.Ready() by {
+//
+//         assert t.Ready();
+//         assert a.Ready();
+//         assert b.Ready();
+//         assert c.Ready();
+//         assert d.Ready();
+//         assert e.Ready();
+//         assert k.Ready();
+//         assert l.Ready();
+//         assert m.Ready();
+//
+//         assert t in os;
+//         assert a in os;
+//         assert b in os;
+//         assert c in os;
+//         assert d in os;
+//         assert e in os;
+//         assert k in os;
+//         assert l in os;
+//         assert m in os;
+//
+//         assert os == {t, a, b, c, d, e, k, l, m};
+//
+//      }
+
+
+    AllTheseFuckingObjectsAreReadyYouIdiot(t, a, b, c, d, e, k, l, m, os);
+
+
+    assert forall x <- os :: x.Ready();
+
+
+
+    print "jandone8\n";
+ }
+
+
+method printAllOwnershipsAndBounds(oo : Owner, context : set<Object>, name : string, mb : Owner := oo)
+//warning - this doesn't do what it should (print stuff out of an object)
+//but prints stuff from the arguments handed in only
+{
+print "============================================================\nprintAllOwnershipsAndBounds ";
+print name, "\n";
+
+print "context= ", ffmtnickset(context), "\n";
+print "oo= ", ffmtnickset(oo), "\n";
+print "flatten(oo)= ", ffmtnickset(flatten(oo)), "\n";
+print "mb= ", ffmtnickset(mb), "\n";
+print "flatten(mb)= ", ffmtnickset(flatten(mb)), "\n";
+print "collectBounds(flatten(oo))= ", ffmtnickset(collectBounds(flatten(oo))), "\n";
+print "set oo.AMFB=", fmtsso( set oo <- flatten(mb) :: oo.AMFB  ), "\n";
+
+print "ctxt>=flatten(oo)= ", (context >= flatten(oo)), "\n";
+print "flatten(oo)>=flatten(mb)= ", (flatten(oo) >= flatten(mb)), "\n";
+print "AllReady(oo)= ", AllReady(oo), "\n";
+print "flatten(mb) >= collectBounds(flatten(oo))= ", flatten(mb) >= collectBounds(flatten(oo)), "\n";
+print "forall oo <- mb :: (flatten(mb) <= oo.AMFB)=", (forall oo <- mb :: (flatten(mb) <= oo.AMFB)) ,"\n";
+}
+
+
+method {:isolate_assertions} sandal8()
+//sets up a full-done clone *with sideways partial owners*
+//otherwise compatible with wrangle - except klone owned by d  from
+//pivot is b, external owner is e, orig is b,c,d, d has owner c & sideowner e, clone is k l m BUT now owned by **d**
+  returns (t : Object, a : Object, b : Object, c : Object, d : Object, e : Object,
+           k : Object, l : Object, m : Object,
+           os : set<Object>, oq : seq<Object>)
+ ensures t.Ready()
+ ensures a.Ready()
+ ensures b.Ready()
+ ensures c.Ready()
+ ensures d.Ready()
+ ensures e.Ready()
+ ensures k.Ready()
+ ensures l.Ready()
+ ensures m.Ready()
+ ensures AllReady(os)
+//  ensures inside(d,c)
+//  ensures inside(d,e)
+ {
+    print "sandal8\n";
+
+    t := new Object.make(protoTypes, {},  {},"t");
+    a := new Object.make(protoTypes, {t}, {t}, "a");
+    b := new Object.make(protoTypes, {a}, {t,a}, "bP");   //pivot
+    c := new Object.make(protoTypes, {b}, {t,a,b}, "c");  //inside clone
+    e := new Object.make(protoTypes, {a}, {t,a}, "eQ");       //external "sideways" owner
+    d := new Object.make(protoTypes, {c,e}, {t,a,b,c,e}, "dX"); //inside pivot and side owner
+
+
+
+assert t.AMFO == {t};
+assert a.AMFO == {t,a};
+assert b.AMFO == {t,a,b};
+assert c.AMFO == {t,a,b,c};
+assert e.AMFO == {t,a,e};
+assert d.AMFO == {t,a,b,c,d,e};
+
+//
+// assert collectAllOwners(t) == {t};
+// assert collectAllOwners(a) == {t,a};
+// assert collectAllOwners(b) == {t,a,b};
+// assert collectAllOwners(c) == {t,a,b,c};
+// assert collectAllOwners(e) == {t,e};
+//
+// assert d.owner == {c,e};
+// assert ({d} + {c,e}) == {c,d,e};
+// assert (set xo <- d.owner, co <- collectAllOwners(xo) :: co) == (collectAllOwners(c) + collectAllOwners(e));
+// var oCE := (collectAllOwners(c) + collectAllOwners(e));
+// assert oCE == (collectAllOwners(c) + collectAllOwners(e)) == ({t,a,b,c} + {t,e}) == {t,a,b,c,e};
+//
+// assert ({d} + d.owner + oCE) ==  {t,a,b,c,d,e};
+// assert collectAllOwners(d) == ({d} + d.owner +  collectAllOwners(c) + collectAllOwners(e)); // == {t,a,b,c,d,e};
+// assert collectAllOwners(d) == {t,a,b,c,d,e};
+//
+//
+
+
+
+
+printAllOwnershipsAndBounds({d}, {t,a,b,c,d,e}, "k¢b");
+
+assert flatten({d}) == {t,a,b,c,d,e};
+            assert {t,a,b,c,d,e} >= flatten({d});
+            assert flatten({d}) >= flatten({d});
+            assert AllReady({d});
+            assert (flatten({d}) >= collectBounds(flatten({d})));
+    k := new Object.make(protoTypes, {d}, {t,a,b,c,d,e}, "k¢b"); //top of coone - of b
+
+/// assert k.AMFO == {t,a,b,c,d,e,k};
+
+printAllOwnershipsAndBounds({k}, {t,a,b,c,d,e,k}, "l¢c");
+
+assume flatten({k}) == {t,a,b,c,d,e,k};
+            assert {t,a,b,c,d,e,k} >= flatten({k});
+            assert flatten({k}) >= flatten({k});
+            assert AllReady({k});
+            assert (flatten({k}) >= collectBounds(flatten({k})));
+    l := new Object.make(protoTypes, {k}, {t,a,b,c,d,e,k}, "l¢c"); //clone of c
+
+/// assert l.AMFO == {t,a,b,c,d,e,k,l};
+
+            var m_context := {t,a,b,c,d,e,k,l};
+            var m_oo := {l,e};
+            var m_mb := m_oo;
+
+            // assert m_context >= flatten(m_oo);
+            // assert flatten(m_oo) >= flatten(m_mb);
+            // assert AllReady(m_oo);
+            // assert (flatten(m_mb) >= collectBounds(flatten(m_oo)));
+
+            assume flatten(m_oo) == {t,a,b,c,d,e,k,l};
+
+            assert m_context >= flatten(m_oo);
+            expect m_context >= flatten(m_oo);
+            assert flatten(m_oo) >= flatten(m_mb);
+            expect flatten(m_oo) >= flatten(m_mb);
+            assert AllReady(m_oo);
+            expect AllReady(m_oo);
+            assert (flatten(m_mb) >= collectBounds(flatten(m_oo)));
+            expect (flatten(m_mb) >= collectBounds(flatten(m_oo)));
+            // assume m_context >= flatten(m_oo) >= flatten(m_mb);
+            // assume AllReady(m_oo);
+            // assume (flatten(m_mb) >= collectBounds(flatten(m_oo)));
+
+printAllOwnershipsAndBounds(m_oo, m_context, "m¢d");
+
+     m := new Object.make(protoTypes, m_oo, m_context, "m¢d"); //clone of d...
+
+
+    os := {t, a, b, c, d, e, k, l, m};
+    oq := [t, a, b, c, d, e, k, l, m];
+
+nl();
+  var x : nat;
+  for x := 0 to |oq| { print fmtamfob(oq[x]), "\n"; }
+nl();
+
+
+
+
+    AllTheseFuckingObjectsAreReadyYouIdiot(t, a, b, c, d, e, k, l, m, os);
+
+
+    assert forall x <- os :: x.Ready();
+
+
+
+    print "sandone8\n";
+ }
+
+
+
+
+
+
+
+
+
+
+
+
+method {:isolate_assertions} randal9()
+//sets up a full-done clone *with sideways partial owners*
+//otherwise compatible with wrangle - except klone owned by d  from
+//pivot is b, external owner is e, orig is b,c,d, d has owner c & sideowner e, clone is k l m BUT now owned by **d**
+  returns (t : Object, a : Object, b : Object, c : Object, d : Object, e : Object,
+           k : Object, l : Object, m : Object,
+           os : set<Object>, oq : seq<Object>)
+ ensures t.Ready()
+ ensures a.Ready()
+ ensures b.Ready()
+ ensures c.Ready()
+ ensures d.Ready()
+ ensures e.Ready()
+ ensures k.Ready()
+ ensures l.Ready()
+ ensures m.Ready()
+ ensures AllReady(os)
+//  ensures inside(d,c)
+//  ensures inside(d,e)
+ {
+    print "randal9 NINE NINE NINE\n";
+
+    t := new Object.make(protoTypes, {},  {},"t");
+    a := new Object.make(protoTypes, {t}, {t}, "a");
+    b := new Object.make(protoTypes, {a}, {t,a}, "b");   //pivot
+    c := new Object.make(protoTypes, {b}, {t,a,b}, "c");  //inside clone
+    e := new Object.make(protoTypes, {a}, {t,a}, "e");       //external "sideways" owner
+    d := new Object.make(protoTypes, {c,e}, {t,a,b,c,e}, "d"); //inside pivot and side owner
+
+
+
+assert t.AMFO == {t};
+assert a.AMFO == {t,a};
+assert b.AMFO == {t,a,b};
+assert c.AMFO == {t,a,b,c};
+assert e.AMFO == {t,a,e};
+assert d.AMFO == {t,a,b,c,d,e};
+
+//
+// assert collectAllOwners(t) == {t};
+// assert collectAllOwners(a) == {t,a};
+// assert collectAllOwners(b) == {t,a,b};
+// assert collectAllOwners(c) == {t,a,b,c};
+// assert collectAllOwners(e) == {t,e};
+//
+// assert d.owner == {c,e};
+// assert ({d} + {c,e}) == {c,d,e};
+// assert (set xo <- d.owner, co <- collectAllOwners(xo) :: co) == (collectAllOwners(c) + collectAllOwners(e));
+// var oCE := (collectAllOwners(c) + collectAllOwners(e));
+// assert oCE == (collectAllOwners(c) + collectAllOwners(e)) == ({t,a,b,c} + {t,e}) == {t,a,b,c,e};
+//
+// assert ({d} + d.owner + oCE) ==  {t,a,b,c,d,e};
+// assert collectAllOwners(d) == ({d} + d.owner +  collectAllOwners(c) + collectAllOwners(e)); // == {t,a,b,c,d,e};
+// assert collectAllOwners(d) == {t,a,b,c,d,e};
+//
+//
+
+
+
+
+printAllOwnershipsAndBounds({d}, {t,a,b,c,d,e}, "k");
+
+assert flatten({d}) == {t,a,b,c,d,e};
+            assert {t,a,b,c,d,e} >= flatten({d});
+            assert flatten({d}) >= flatten({d});
+            assert AllReady({d});
+            assert (flatten({d}) >= collectBounds(flatten({d})));
+    k := new Object.make(protoTypes, {d}, {t,a,b,c,d,e}, "k"); //top of coone - of b
+
+/// assert k.AMFO == {t,a,b,c,d,e,k};
+
+printAllOwnershipsAndBounds({k}, {t,a,b,c,d,e,k}, "l");
+
+assume flatten({k}) == {t,a,b,c,d,e,k};
+            assert {t,a,b,c,d,e,k} >= flatten({k});
+            assert flatten({k}) >= flatten({k});
+            assert AllReady({k});
+            assert (flatten({k}) >= collectBounds(flatten({k})));
+    l := new Object.make(protoTypes, {k}, {t,a,b,c,d,e,k}, "l"); //clone of c
+
+/// assert l.AMFO == {t,a,b,c,d,e,k,l};
+
+            var m_context := {t,a,b,c,d,e,k,l};
+            var m_oo := {l,e};
+            var m_mb := m_oo;
+
+            // assert m_context >= flatten(m_oo);
+            // assert flatten(m_oo) >= flatten(m_mb);
+            // assert AllReady(m_oo);
+            // assert (flatten(m_mb) >= collectBounds(flatten(m_oo)));
+
+            assume flatten(m_oo) == {t,a,b,c,d,e,k,l};
+
+            assert m_context >= flatten(m_oo);
+            expect m_context >= flatten(m_oo);
+            assert flatten(m_oo) >= flatten(m_mb);
+            expect flatten(m_oo) >= flatten(m_mb);
+            assert AllReady(m_oo);
+            expect AllReady(m_oo);
+            assert (flatten(m_mb) >= collectBounds(flatten(m_oo)));
+            expect (flatten(m_mb) >= collectBounds(flatten(m_oo)));
+            // assume m_context >= flatten(m_oo) >= flatten(m_mb);
+            // assume AllReady(m_oo);
+            // assume (flatten(m_mb) >= collectBounds(flatten(m_oo)));
+
+printAllOwnershipsAndBounds(m_oo, m_context, "m");
+
+     m := new Object.make(protoTypes, m_oo, m_context, "m"); //clone of d...
+
+
+    os := {t, a, b, c, d, e, k, l, m};
+    oq := [t, a, b, c, d, e, k, l, m];
+//
+// nl();
+//   var x : nat;
+//   for x := 0 to |oq| { print fmtamfob(oq[x]), "\n"; }
+// nl();
+
+
+
+
+    AllTheseFuckingObjectsAreReadyYouIdiot(t, a, b, c, d, e, k, l, m, os);
+
+
+    assert forall x <- os :: x.Ready();
+
+
+
+    print "randone9\n";
+ }
+
+
+
+
+
+
+
+
+
+
+method {:isolate_assertions} zandal9()
+//sets up a single "column" of objects to show permissible links - five objects, t, a..d
+//in this version, all boundaries == owners
+  returns (t : Object, a : Object, b : Object, c : Object, d : Object, e : Object,
+           k : Object, l : Object, m : Object,
+           os : set<Object>, oq : seq<Object>, loutName : string)
+ ensures t.Ready()
+ ensures a.Ready()
+ ensures b.Ready()
+ ensures c.Ready()   //should be the centre
+ ensures d.Ready()
+ ensures e.Ready()
+ ensures k.Ready()
+ ensures l.Ready()
+ ensures m.Ready()
+ ensures AllReady(os)
+//  ensures inside(d,c)
+//  ensures inside(d,e)
+ {
+    loutName := "zandall9";
+    print loutName, " NINE NINE NINE\n";
+
+
+      t := new Object.make(protoTypes, {},  {},"t");
+      a := new Object.make(protoTypes, {t}, {t}, "a");
+      b := new Object.make(protoTypes, {a}, {t,a}, "b");
+      c := new Object.make(protoTypes, {b}, {t,a,b}, "c");
+      d := new Object.make(protoTypes, {c}, {t,a,b,c}, "d");
+      e := new Object.make(protoTypes, {d}, {t,a,b,c,d}, "e");
+
+
+
+printAllOwnershipsAndBounds({},  {},"t");
+printAllOwnershipsAndBounds({t}, {t}, "a");
+printAllOwnershipsAndBounds({a}, {t,a}, "b");
+printAllOwnershipsAndBounds({b}, {t,a,b}, "c");
+printAllOwnershipsAndBounds({c}, {t,a,b,c}, "d");
+printAllOwnershipsAndBounds({d}, {t,a,b,c,d}, "e");
+
+
+assert t.AMFO == {t};
+assert a.AMFO == {t,a};
+assert b.AMFO == {t,a,b};
+assert c.AMFO == {t,a,b,c};
+assert d.AMFO == {t,a,b,c,d};
+assert e.AMFO == {t,a,b,c,d,e};
+
+k := t; l := t; m := t;
+
+    os := {t, a, b, c, d, e};
+    oq := [t, a, b, c, d, e];
+
+    print "zandall9 no boundary \n";
+  }
+
+
+
+
+
+
+
+
+method {:isolate_assertions} zandal9bounded()
+//sets up a single "column" of objects to show permissible links - five objects, t,a..d, with c & d boundary pushed up to a.
+//
+  returns (t : Object, a : Object, b : Object, c : Object, d : Object, e : Object,
+           k : Object, l : Object, m : Object,
+           os : set<Object>, oq : seq<Object>, loutName : string)
+ ensures t.Ready()
+ ensures a.Ready()
+ ensures b.Ready()
+ ensures c.Ready()   //should be the centre
+ ensures d.Ready()
+ ensures e.Ready()
+ ensures k.Ready()
+ ensures l.Ready()
+ ensures m.Ready()
+ ensures AllReady(os)
+//  ensures inside(d,c)
+//  ensures inside(d,e)
+ {
+    loutName := "zandall9bounded";
+    print loutName, " NINE NINE NINE\n";
+
+
+      t := new Object.make(protoTypes, {},  {},"t");
+      a := new Object.make(protoTypes, {t}, {t}, "a");
+      b := new Object.make(protoTypes, {a}, {t,a}, "b");
+      c := new Object.make(protoTypes, {b}, {t,a,b}, "c", {a});
+      d := new Object.make(protoTypes, {c}, {t,a,b,c}, "d", {a});
+      e := new Object.make(protoTypes, {d}, {t,a,b,c,d}, "e", {a});
+
+
+
+printAllOwnershipsAndBounds({},  {},"t");
+printAllOwnershipsAndBounds({t}, {t}, "a");
+printAllOwnershipsAndBounds({a}, {t,a}, "b");
+printAllOwnershipsAndBounds({b}, {t,a,b}, "c");
+printAllOwnershipsAndBounds({c}, {t,a,b,c}, "d", {a});
+printAllOwnershipsAndBounds({d}, {t,a,b,c,d}, "e", {a});
+
+
+assert t.AMFO == {t};
+assert a.AMFO == {t,a};
+assert b.AMFO == {t,a,b};
+assert c.AMFO == {t,a,b,c};
+assert d.AMFO == {t,a,b,c,d};
+assert e.AMFO == {t,a,b,c,d,e};
+
+k := t; l := t; m := t;
+
+    os := {t, a, b, c, d, e};
+    oq := [t, a, b, c, d, e];
+
+    print "zandl9bounded";
+
+    return;
+
+printAllOwnershipsAndBounds({t}, {t,a,b,c,d,e}, "k");
+
+//          {t}, {t,a,b,c,d,e}, "k");
+
+// assert flatten({d}) == {t,a,b,c,d,e};
+//             assert {t,a,b,c,d,e} >= flatten({d});
+//             assert flatten({d}) >= flatten({d});
+//             assert AllReady({d});
+//             assert (flatten({d}) >= collectBounds(flatten({d})));
+    k := new Object.make(protoTypes, {t}, {t,a,b,c,d,e}, "k");
+
+/// assert k.AMFO == {t,a,b,c,d,e,k};
+
+printAllOwnershipsAndBounds({a}, {t,a,b,c,d,e,k}, "l");
+
+assume flatten({k}) == {t,k};
+            assert AllReady({k});
+            assert (flatten({k}) >= collectBounds(flatten({k})));
+    l := new Object.make(protoTypes, {a}, {t,a,b,c,d,e,k}, "l");
+
+/// assert l.AMFO == {t,a,b,c,d,e,k,l};
+
+            var m_context := {t,a,b,c,d,e,k,l};
+            var m_oo := {b};
+            var m_mb := m_oo;
+
+            // assert m_context >= flatten(m_oo);
+            // asse rt flatten(m_oo) >= flatten(m_mb);
+            // assert AllReady(m_oo);
+            // assert (flatten(m_mb) >= collectBounds(flatten(m_oo)));
+
+ //            assume flatten(m_oo) == {t,a,b,c,d,e,k,l};  //IF m_oo  == {b}?  WTF???
+
+            // these assert/expect pairs used to work but now the don't.  WHY?
+            // assert m_context >= flatten(m_oo);
+            // expect m_context >= flatten(m_oo);
+            // assert flatten(m_oo) >= flatten(m_mb);
+            // expect flatten(m_oo) >= flatten(m_mb);
+            // assert AllReady(m_oo);
+            // expect AllReady(m_oo);
+            // assert (flatten(m_mb) >= collectBounds(flatten(m_oo)));
+            // expect (flatten(m_mb) >= collectBounds(flatten(m_oo)));
+
+            // // assume m_context >= flatten(m_oo) >= flatten(m_mb);
+            // // assume AllReady(m_oo);
+            // // assume (flatten(m_mb) >= collectBounds(flatten(m_oo)));
+
+printAllOwnershipsAndBounds(m_oo, m_context, "m");
+
+     m := new Object.make(protoTypes, m_oo, m_context, "m"); //clone of d...
+
+
+    os := {t, a, b, c, d, e, k, l, m};
+    oq := [t, a, b, c, d, e, k, l, m];
+
+
+    print "zandlone9bounded\n";
+   }
+
+
+
+
+
+
+
+
+lemma {:isolate_assertions} {:timeLimit 60} AllTheseFuckingObjectsAreReadyYouIdiot(
+    t : Object,
+    a : Object, b : Object, c : Object, d : Object, e : Object,
+    k : Object, l : Object, m : Object,
+    os : set<Object>)
+
+        requires t.Ready()
+        requires a.Ready()
+        requires b.Ready()
+        requires c.Ready()
+        requires d.Ready()
+        requires e.Ready()
+        requires k.Ready()
+        requires l.Ready()
+        requires m.Ready()
+
+        // requires t in os
+        // requires a in os
+        // requires b in os
+        // requires c in os
+        // requires d in os
+        // requires e in os
+        // requires k in os
+        // requires l in os
+        // requires m in os
+
+        requires os == {t, a, b, c, d, e, k, l, m}
+
+        ensures forall x <- os :: x.Ready()
+{
+        // assert t.Ready();
+        // assert a.Ready();
+        // assert b.Ready();
+        // assert c.Ready();
+        // assert d.Ready();
+        // assert e.Ready();
+        // assert k.Ready();
+        // assert l.Ready();
+        // assert m.Ready();
+
+        // assert t in os;
+        // assert a in os;
+        // assert b in os;
+        // assert c in os;
+        // assert d in os;
+        // assert e in os;
+        // assert k in os;
+        // assert l in os;
+        // assert m in os;
+
+        // assert os == {t, a, b, c, d, e, k, l, m};
+
+        // assert forall x <- os :: x.Ready();
+}
+
+
+method {:isolate_assertions} zandal0()
+  //easier than declaring everything in main
+  returns (t : Object, a : Object, b : Object, c : Object, d : Object, e : Object,
+           k : Object, l : Object, m : Object,
+           os : set<Object>, oq : seq<Object>, loutName : string)
+ ensures t.Ready()
+ ensures a.Ready()
+ ensures b.Ready()
+ ensures c.Ready()   //should be the centre
+ ensures d.Ready()
+ ensures e.Ready()
+ ensures k.Ready()
+ ensures l.Ready()
+ ensures m.Ready()
+ ensures AllReady(os)
+ {
+    loutName := "NOTHING";
+    t := new Object.make(protoTypes, {},  {},"t");
+    a := t;
+    b := t;
+    c := t;
+    d := t;
+    e := t;
+    k := t;
+    l := t;
+    m := t;
+    os := {t, a, b, c, d, e, k, l, m};
+    oq := [t, a, b, c, d, e, k, l, m];
+ }
+
+
+
+method {:isolate_assertions} zandalList()
+  //easier than declaring everything in main
+  returns (t : Object, a : Object, b : Object, c : Object, d : Object, e : Object,
+           k : Object, l : Object, m : Object,
+           os : set<Object>, oq : seq<Object>, loutName : string)
+ ensures t.Ready()
+ ensures a.Ready()
+ ensures b.Ready()
+ ensures c.Ready()   //should be the centre
+ ensures d.Ready()
+ ensures e.Ready()
+ ensures k.Ready()
+ ensures l.Ready()
+ ensures m.Ready()
+ ensures AllReady(os)
+ {
+
+
+var list  := new Object.make(fields({"head", "tail"}), {}, {}, "list")        ;
+
+var link0 := new Object.make(fields({"next", "data"}), {list}, {list}, "link0", {} );
+var link1 := new Object.make(fields({"next", "data"}), {list}, {list}, "link1", {} );
+var link2 := new Object.make(fields({"next", "data"}), {list}, {list}, "link2", {} );
+var link3 := new Object.make(fields({"next", "data"}), {list}, {list}, "link3", {} );
+
+var elem0 := new Object.make(fields({}), {}, {list}, "elem0", {} );
+var elem1 := new Object.make(fields({}), {}, {list}, "elem1", {} );
+var elem2 := new Object.make(fields({}), {}, {list}, "elem2", {} );
+var elem3 := new Object.make(fields({}), {}, {list}, "elem3", {} );
+
+
+ list.setf("head", link0); //list.setf("tail", link3);
+
+ link0.setf("next", link1); link1.setf("next", link2); link2.setf("next", link3);
+ link0.setf("data", elem0); link1.setf("data", elem1); link2.setf("data", elem2); link3.setf("data", elem3);
+
+
+    loutName := "LINKED LIST";
+    t := elem3;
+    a := list;
+    b := link0;
+    c := link1;
+    d := link2;
+    e := link3;
+    k := elem0;
+    l := elem1;
+    m := elem2;
+    os := {t, a, b, c, d, e, k, l, m};
+    oq := [t, a, b, c, d, e, k, l, m];
+ }
+
+
+
+
+
+
+
+
+
+
+
+
+
+
+
+
+const listF : map<string, Mode> := fields({"head"})
+const linkF : map<string, Mode> := fields({"data","next"})
+const frame : map<string, Mode> := fields({"a","b","c"})
+const appData := frame
+
+method {:isolate_assertions} zandal10()
+//sets up a two "columns" of objects to show permissible links - five objects, t, a..e
+//in this version, all boundaries == owners
+  returns (t : Object, a : Object, b : Object, c : Object, d : Object, e : Object,
+           k : Object, l : Object, m : Object,
+           os : set<Object>, oq : seq<Object>, loutName : string)
+ ensures t.Ready()
+ ensures a.Ready()
+ ensures b.Ready()
+ ensures c.Ready()   //should be the centre
+ ensures d.Ready()
+ ensures e.Ready()
+ ensures k.Ready()
+ ensures l.Ready()
+ ensures m.Ready()
+ ensures AllReady(os)
+
+ {
+    loutName := "zandal10";
+    print loutName, " NINE NINE NINE\n";
+
+
+//bugger it - rewally should move the OWNER to thw front sbhojldnb't I
+//and get rid of fields
+      t := new Object.make(frame, {},  {},"3");
+      a := new Object.make(frame, {t}, {t}, "2");
+      b := new Object.make(frame, {a}, {t,a}, "1");
+      k := new Object.make(frame, {b}, {t,a,b}, "0");
+
+      m := new Object.make(appData, {t}, {t}, "S");
+
+      l := new Object.make(listF, {b}, {t}, "L");
+      c := new Object.make(linkF, {l}, {t,a,b,k,l,m}, "i");
+      d := new Object.make(linkF, {l}, {t,a,b,c,k,l,m}, "j");
+
+      e := new Object.make(protoTypes, {k,l}, {t,a,b,c,d,k,l,m}, "00");
+
+    t.setf("s",m);
+    b.setf(",",l);
+    l.setf("head",c);
+    c.setf("next",d);
+
+
+    os := {t, a, b, c, d, e, k, l, m};
+    oq := [t, a, b, c, d, e, k, l, m];
+
+    print "zandal10";
+  }
+
+
+
+
+
+
+
+method {:isolate_assertions} zandal11()
+//sets up a two "columns" of objects to show permissible links - five objects, t, a..e
+//in this version, all boundaries == owners
+  returns (t : Object, a : Object, b : Object, c : Object, d : Object, e : Object,
+           k : Object, l : Object, m : Object,
+           os : set<Object>, oq : seq<Object>, loutName : string)
+ ensures t.Ready()
+ ensures a.Ready()
+ ensures b.Ready()
+ ensures c.Ready()   //should be the centre
+ ensures d.Ready()
+ ensures e.Ready()
+ ensures k.Ready()
+ ensures l.Ready()
+ ensures m.Ready()
+ ensures AllReady(os)
+
+ {
+    loutName := "zandal10";
+    print loutName, " NINE NINE NINE\n";
+
+
+//bugger it - rewally should move the nickname to thw front sbhojldnb't I
+      t := new Object.make(protoTypes, {},  {},"t");
+      a := new Object.make(protoTypes, {t}, {t}, "a");
+      b := new Object.make(protoTypes, {a}, {t,a}, "b");
+
+      k := new Object.make(protoTypes, {t}, {t}, "k");
+      l := new Object.make(protoTypes, {k}, {t,k}, "l");
+      m := new Object.make(protoTypes, {l}, {t,k,l}, "m");
+
+      c := new Object.make(protoTypes, {b,m}, {t,a,b,k,l,m}, "c");
+      d := new Object.make(protoTypes, {c},   {t,a,b,c,k,l,m}, "d");
+      e := new Object.make(protoTypes, {d},   {t,a,b,c,d,k,l,m}, "e");
+
+
+
+
+
+printAllOwnershipsAndBounds({},  {},"t");
+printAllOwnershipsAndBounds({t}, {t}, "a");
+printAllOwnershipsAndBounds({a}, {t,a}, "b");
+
+printAllOwnershipsAndBounds({t}, {t}, "k");
+printAllOwnershipsAndBounds({k}, {t,k}, "l");
+printAllOwnershipsAndBounds({l}, {t,k,l}, "m");
+
+printAllOwnershipsAndBounds({b}, {t,a,b,k,l,m}, "c");
+printAllOwnershipsAndBounds({c}, {t,a,b,c,k,l,m}, "d");
+printAllOwnershipsAndBounds({d}, {t,a,b,c,d,k,l,m}, "e");
+
+
+assert t.AMFO == {t};
+assert a.AMFO == {t,a};
+assert b.AMFO == {t,a,b};
+
+assert k.AMFO == {t,k};
+assert l.AMFO == {t,k,l};
+assert m.AMFO == {t,k,l,m};
+
+assert c.AMFO == {t,a,b,c};
+assert d.AMFO == {t,a,b,c,d};
+assert e.AMFO == {t,a,b,c,d,e};
+
+
+    os := {t, a, b, c, d, e, k, l, m};
+    oq := [t, a, b, c, d, e, k, l, m];
+
+    print "zandal10";
+  }
+
+
+
+
+
+
+lemma {:isolate_assertions} {:timeLimit 60} AllTheseFuckingObjectsAreReadyYouIdiotVarargs(
+    os : set<Object>, t : Object,
+     a : Object := t, b : Object := t, c : Object := t, d : Object := t, e : Object := t,
+     k : Object := t, l : Object := t, m : Object := t)
+
+        requires t.Ready()
+        requires a.Ready()
+        requires b.Ready()
+        requires c.Ready()
+        requires d.Ready()
+        requires e.Ready()
+        requires k.Ready()
+        requires l.Ready()
+        requires m.Ready()
+
+        // requires t in os
+        // requires a in os
+        // requires b in os
+        // requires c in os
+        // requires d in os
+        // requires e in os
+        // requires k in os
+        // requires l in os
+        // requires m in os
+
+        requires os == {t, a, b, c, d, e, k, l, m}
+
+        ensures forall x <- os :: x.Ready()
+
+        {}
+
+
+
+
+
+
+
+
+
+
+
+
+
+
+
+
+
+
+
+
+
+
+
+
+
+
+
+
+
+
+
+
+
+
+
+
+
+
+
+
+
+
+
+
+
+
+
+
+
+
+
+
+
+
+
+
+
+
+
+
+
+
+
+
+
+
+
+
+
+
+
+
+
+
+
+
+
+
+
+
+
+
+
+
+
+
+
+
+
+
+
+
+
+
+
+
+
+
+
+
+
+
+
+
+
+
+
+
+
+
+
+
+
+
+
+
+
+
+
+
+
+
+
+
+const owner_attrs := "[arrowhead=diamond,penwidth=3,weight=10,layer=owner]"
+
+const nowner_attrs := "[arrowhead=none,penwidth=0,weight=10,layer=bg]"
+
+const bound_attrs := "[arrowhead=diamond,penwidth=3,weight=10,layer=bound,color=pink,constraint=false]"
+const AMFO_attrs := "[penwidth=0.1,layer=amfo,weight=1,arrowhead=invempty,constraint=false]"
+const AMFB_attrs := "[penwidth=0.1,layer=amfo,weight=1,arrowhead=invempty,constraint=false, color=pink]"
+const mapping_attrs := "[penwidth=2,layer=mapping,weight=0,color=blue,constraint=false]"
+
+const refOKOattrs := "[penwidth=2,layer=mapping,weight=0,color=green,constraint=false]"  //both
+const refOO_attrs := "[penwidth=2,layer=mapping,weight=0,color=orange,constraint=false,style=dashed]" //  label=O
+const refOK_attrs := "[penwidth=2,layer=mapping,weight=0,color=purple ,constraint=false]"
+const refNK_attrs := "[penwidth=2,layer=mapping,weight=0,color=red,constraint=false,style=dashed]"  //label=\"X\", fontname=Helvetica,fontsize=30,fontcolor=red,labelOverlay=\"true\"
+
+
+const field_attrs := "[penwidth=1,layer=fields,weight=0.5,fontsize=9,arrowhead=normal]"
+
+method {:verify false}  graphobjectset(s : set<Object>, m : Klon, pops : PrintOptions)
+{
+  var o := s;
+
+  while o != {}
+    decreases o
+  {
+    var y: Object;
+    y :| y in o;
+    graphobject(y, pops);
+//    print "- - - - - - - -\n";
+    o := o - {y};
+  }
+
+}
+
+
+
+
+
+
+method {:verify false}  graphobject(o : Object, pops : PrintOptions)
+{
+  //ownership
+
+  print "\n//object ";
+  print o.nick, "\n";
+
+  var oo := o.owner;
+
+  while oo != {}
+    decreases oo
+  {
+    var y: Object;
+    y :| y in oo;
+
+  if pops.lineOpt('O') { print o.nick, " -> ", y.nick, " ", owner_attrs, "\n"; }
+     else { print o.nick, " -> ", y.nick, " ", nowner_attrs, "\n"; }
+
+
+    oo := oo - {y};
+  }
+
+  oo := o.AMFO;
+
+  while oo != {}
+    decreases oo
+  {
+    var y: Object;
+    y :| y in oo;
+
+   if pops.lineOpt('o') {
+       if (o != y) { print o.nick, " -> ", y.nick, " ", AMFO_attrs, "\n"; }
+   }
+
+    oo := oo - {y};
+  }
+
+
+
+/////////////////////////
+///same as above for bounds.  need to do better than cut & paste  (why?)
+
+   oo := o.bound;
+
+  while oo != {}
+    decreases oo
+  {
+    var y: Object;
+    y :| y in oo;
+
+ if pops.lineOpt('B')
+      {  print o.nick, " -> ", y.nick, " ", bound_attrs, "\n"; }
+
+    oo := oo - {y};
+  }
+
+  oo := o.AMFB;
+
+  while oo != {}
+    decreases oo
+  {
+    var y: Object;
+    y :| y in oo;
+
+//   if ((o != y) && (y !in o.AMFB))
+    if pops.lineOpt('b') { print o.nick, " -> ", y.nick, " ", AMFB_attrs, "\n"; }
+
+    oo := oo - {y};
+  }
+
+////////////////////////////
+
+ if  (not(pops.lineOpt('F'))) { return; }
+
+  var fs := o.fields.Keys;
+
+  while fs != {}
+    decreases fs
+  {
+    var f: string;
+    f :| f in fs;
+
+    var nf := o.nick;
+    var nt := o.fields[f].nick;
+    if (pops.nodeOpt(nf) || pops.nodeOpt(nt)) {
+            print nf, " -> ", nt,     " ", field_attrs;
+            print "[label=\"", f, "\"]";
+            if (f == "contents") { print "[weight=2.5]"; }
+            if (f == "next") { print "[weight=5]"; }
+            print "\n";
+        }
+    fs := fs - {f};
+  }
+
+}
+
+
+
+
+
+
+method graphmapping(m : vmap<Object,Object>, pops : PrintOptions)
+  modifies {}
+  ensures unchanged(m.Keys,m.Values)
+  ensures forall k <- m.Keys   :: unchanged(k)
+  ensures forall v <- m.Values :: unchanged(v)
+{
+
+  print "\n\n//mapping\n";
+  var t := m;
+  while t != map[]
+    decreases t
+  {
+    var y: Object;
+    y :| y in t.Keys;
+    print y.nick, " -> ", t[y].nick, " ", mapping_attrs, "\n";
+    t := t - {y};
+  }
+}
+
+
+
+method graphrefs(s : seq<Object>, pops : PrintOptions)
+  modifies {}
+{
+  print "\n\n//refs\n";
+
+    for f := 0 to |s| {
+      for t := 0 to |s| {
+  //       var attrs := if (refOK(s[f],s[t])) then refOK_attrs else refNK_attrs;
+
+          var attrs := refNK_attrs; //not permitted reference - red, X
+          if  (refOK(s[f],s[t])) { attrs := refOK_attrs; } //reference permitted w/ boundary - but not without (purple,. shouldn't happen)
+          if  (refOO(s[f],s[t])) { attrs := refOO_attrs; } //reference without w/ boundary - but NOT permitted with bounday - ORANGE, "O"
+          if ((refOK(s[f],s[t])) && (refOO(s[f],s[t]))) { attrs := refOKOattrs; } //OK either way - GREEN
+
+
+//      if ((s[f].nick == "c") || (s[t].nick == "c"))
+//    if (attrs != refNK_attrs) && (s[f].nick in {"a", "b", "c", "d", "e"})
+//    if (s[f].nick in {"c", "d", "e"})
+
+     if (pops.nodeOpt(s[f].nick) || pops.nodeOpt(s[t].nick))
+        {
+        print s[f].nick, " -> ", s[t].nick, " ", attrs, "\n";
+       }
+    }
+   }
+}
+
+
+method printrefs(s : seq<Object>)
+  modifies {}
+{
+  print "PRINTREFS-------------------------------------\n";
+
+    for f := 0 to |s| {
+      for t := 0 to |s| {
+           print s[f].nick, " -> ", s[t].nick, "  ";
+
+           print if (s[f]==s[t]) then "== " else "   ";
+           print if (refDI(s[f],s[t])) then "D " else "  ";
+           print if (refBI(s[f],s[t])) then "B " else "  ";
+           print if (refOI(s[f],s[t])) then "O " else "  ";
+           print if (refOO(s[f],s[t])) then "OO " else "   ";
+           print if (refOK(s[f],s[t])) then "OK " else "   ";
+
+           nl();
+      }
+    }
+}
